Move auxiliary lemmata out of SafeConversion

pcuic/theories/PCUICSafeConversion.v
@@ -6,7 +6,7 @@ From Template Require Import config Universes monad_utils utils BasicAst
      AstUtils UnivSubst.
 From PCUIC Require Import PCUICAst PCUICAstUtils PCUICInduction PCUICReflect
      PCUICLiftSubst PCUICUnivSubst PCUICTyping PCUICSafeReduce PCUICCumulativity
-     PCUICSR PCUICPosition PCUICEquality PCUICNameless.
+     PCUICSR PCUICPosition PCUICEquality PCUICNameless PCUICSafeLemmata.
 From Equations Require Import Equations.
 
 Require Import Equations.Prop.DepElim.
@@ -22,443 +22,13 @@ Module PSR := PCUICSafeReduce.
 
  *)
 
-Inductive conv_pb :=
-| Conv
-| Cumul.
-
 Section Conversion.
 
   Context (flags : RedFlags.t).
   Context (Σ : global_context).
   Context (hΣ : wf Σ).
 
-  Tactic Notation "zip" "fold" "in" hyp(h) :=
-    lazymatch type of h with
-    | context C[ zipc ?t ?π ] =>
-      let C' := context C[ zip (t,π) ] in
-      change C' in h
-    end.
-
-  Tactic Notation "zip" "fold" :=
-    lazymatch goal with
-    | |- context C[ zipc ?t ?π ] =>
-      let C' := context C[ zip (t,π) ] in
-      change C'
-    end.
-
-  Definition conv leq Σ Γ u v :=
-    match leq with
-    | Conv => ∥ Σ ;;; Γ |- u = v ∥
-    | Cumul => ∥ Σ ;;; Γ |- u <= v ∥
-    end.
-
-  Definition nodelta_flags := RedFlags.mk true true true false true true.
-
-  Lemma welltyped_rename :
-    forall Γ u v,
-      welltyped Σ Γ u ->
-      eq_term (snd Σ) u v ->
-      welltyped Σ Γ v.
-  Admitted.
-
-  Lemma red_welltyped :
-    forall {Γ u v},
-      welltyped Σ Γ u ->
-      ∥ red (fst Σ) Γ u v ∥ ->
-      welltyped Σ Γ v.
-  Proof.
-    intros Γ u v h [r].
-    revert h. induction r ; intros h.
-    - assumption.
-    - specialize IHr with (1 := ltac:(eassumption)).
-      destruct IHr as [A ?]. exists A.
-      eapply PSR.subject_reduction ; eassumption.
-  Qed.
-
-  Lemma red_cored_or_eq :
-    forall Γ u v,
-      red Σ Γ u v ->
-      cored Σ Γ v u \/ u = v.
-  Proof.
-    intros Γ u v h.
-    induction h.
-    - right. reflexivity.
-    - destruct IHh.
-      + left. eapply cored_trans ; eassumption.
-      + subst. left. constructor. assumption.
-  Qed.
-
   Set Equations With UIP.
-
-  Lemma cored_it_mkLambda_or_LetIn :
-    forall Γ Δ u v,
-      cored Σ (Γ ,,, Δ) u v ->
-      cored Σ Γ (it_mkLambda_or_LetIn Δ u)
-               (it_mkLambda_or_LetIn Δ v).
-  Proof.
-    intros Γ Δ u v h.
-    induction h.
-    - constructor. apply red1_it_mkLambda_or_LetIn. assumption.
-    - eapply cored_trans.
-      + eapply IHh.
-      + apply red1_it_mkLambda_or_LetIn. assumption.
-  Qed.
-
-  Lemma red_it_mkLambda_or_LetIn :
-    forall Γ Δ u v,
-      red Σ (Γ ,,, Δ) u v ->
-      red Σ Γ (it_mkLambda_or_LetIn Δ u)
-              (it_mkLambda_or_LetIn Δ v).
-  Proof.
-    intros Γ Δ u v h.
-    induction h.
-    - constructor.
-    - econstructor.
-      + eassumption.
-      + eapply red1_it_mkLambda_or_LetIn. assumption.
-  Qed.
-
-  Lemma cored_zipx :
-    forall Γ u v π,
-      cored Σ (Γ ,,, stack_context π) u v ->
-      cored Σ [] (zipx Γ u π) (zipx Γ v π).
-  Proof.
-    intros Γ u v π h.
-    eapply cored_it_mkLambda_or_LetIn.
-    eapply cored_context.
-    rewrite app_context_nil_l.
-    assumption.
-  Qed.
-
-  Lemma red_zipx :
-    forall Γ u v π,
-      red Σ (Γ ,,, stack_context π) u v ->
-      red Σ [] (zipx Γ u π) (zipx Γ v π).
-  Proof.
-    intros Γ u v π h.
-    eapply red_it_mkLambda_or_LetIn.
-    eapply red_context.
-    rewrite app_context_nil_l.
-    assumption.
-  Qed.
-
-  Lemma red_trans :
-    forall Γ u v w,
-      red (fst Σ) Γ u v ->
-      red (fst Σ) Γ v w ->
-      red (fst Σ) Γ u w.
-  Proof.
-    intros Γ u v w h1 h2.
-    revert u h1. induction h2 ; intros u h1.
-    - assumption.
-    - specialize IHh2 with (1 := h1).
-      eapply trans_red.
-      + eapply IHh2.
-      + assumption.
-  Qed.
-
-  Lemma conv_refl' :
-    forall leq Γ t,
-      conv leq Σ Γ t t.
-  Proof.
-    intros leq Γ t.
-    destruct leq.
-    - cbn. constructor. apply conv_refl.
-    - cbn. constructor. apply cumul_refl'.
-  Qed.
-
-  Lemma conv_sym :
-    forall Γ u v,
-      Σ ;;; Γ |- u = v ->
-      Σ ;;; Γ |- v = u.
-  Proof.
-    intros Γ u v [h1 h2].
-    econstructor ; assumption.
-  Qed.
-
-  Lemma conv_conv :
-    forall {Γ leq u v},
-      ∥ Σ ;;; Γ |- u = v ∥ ->
-      conv leq Σ Γ u v.
-  Proof.
-    intros Γ leq u v h.
-    destruct leq.
-    - assumption.
-    - destruct h as [[h1 h2]]. cbn.
-      constructor. assumption.
-  Qed.
-
-  Lemma eq_term_conv :
-    forall {Γ u v},
-      eq_term (snd Σ) u v ->
-      Σ ;;; Γ |- u = v.
-  Proof.
-    intros Γ u v e.
-    constructor.
-    - eapply cumul_refl.
-      eapply eq_term_leq_term. assumption.
-    - eapply cumul_refl.
-      eapply eq_term_leq_term.
-      eapply eq_term_sym.
-      assumption.
-  Qed.
-
-  Lemma conv_trans :
-    forall Γ u v w,
-      Σ ;;; Γ |- u = v ->
-      Σ ;;; Γ |- v = w ->
-      Σ ;;; Γ |- u = w.
-  Proof.
-    intros Γ u v w h1 h2.
-    destruct h1, h2. constructor ; eapply cumul_trans ; eassumption.
-  Qed.
-
-  Lemma conv_trans' :
-    forall leq Γ u v w,
-      conv leq Σ Γ u v ->
-      conv leq Σ Γ v w ->
-      conv leq Σ Γ u w.
-  Proof.
-    intros leq Γ u v w h1 h2.
-    destruct leq.
-    - cbn in *. destruct h1, h2. constructor.
-      eapply conv_trans ; eassumption.
-    - cbn in *. destruct h1, h2. constructor. eapply cumul_trans ; eassumption.
-  Qed.
-
-  Lemma red_conv_l :
-    forall leq Γ u v,
-      red (fst Σ) Γ u v ->
-      conv leq Σ Γ u v.
-  Proof.
-    intros leq Γ u v h.
-    induction h.
-    - apply conv_refl'.
-    - eapply conv_trans' ; try eassumption.
-      destruct leq.
-      + simpl. constructor. constructor.
-        * eapply cumul_red_l.
-          -- eassumption.
-          -- eapply cumul_refl'.
-        * eapply cumul_red_r.
-          -- eapply cumul_refl'.
-          -- assumption.
-      + simpl. constructor.
-        eapply cumul_red_l.
-        * eassumption.
-        * eapply cumul_refl'.
-  Qed.
-
-  Lemma red_conv_r :
-    forall leq Γ u v,
-      red (fst Σ) Γ u v ->
-      conv leq Σ Γ v u.
-  Proof.
-    intros leq Γ u v h.
-    induction h.
-    - apply conv_refl'.
-    - eapply conv_trans' ; try eassumption.
-      destruct leq.
-      + simpl. constructor. constructor.
-        * eapply cumul_red_r.
-          -- eapply cumul_refl'.
-          -- assumption.
-        * eapply cumul_red_l.
-          -- eassumption.
-          -- eapply cumul_refl'.
-      + simpl. constructor.
-        eapply cumul_red_r.
-        * eapply cumul_refl'.
-        * assumption.
-  Qed.
-
-  Lemma conv_conv_l :
-    forall leq Γ u v,
-        Σ ;;; Γ |- u = v ->
-        conv leq Σ Γ u v.
-  Proof.
-    intros [] Γ u v [h1 h2].
-    - cbn. constructor. constructor ; assumption.
-    - cbn. constructor. assumption.
-  Qed.
-
-  Lemma conv_conv_r :
-    forall leq Γ u v,
-        Σ ;;; Γ |- u = v ->
-        conv leq Σ Γ v u.
-  Proof.
-    intros [] Γ u v [h1 h2].
-    - cbn. constructor. constructor ; assumption.
-    - cbn. constructor. assumption.
-  Qed.
-
-  Lemma cumul_App_l :
-    forall {Γ f g x},
-      Σ ;;; Γ |- f <= g ->
-      Σ ;;; Γ |- tApp f x <= tApp g x.
-  Proof.
-    intros Γ f g x h.
-    induction h.
-    - eapply cumul_refl. constructor.
-      + assumption.
-      + apply leq_term_refl.
-    - eapply cumul_red_l ; try eassumption.
-      econstructor. assumption.
-    - eapply cumul_red_r ; try eassumption.
-      econstructor. assumption.
-  Qed.
-
-  Lemma conv_App_r :
-    forall {Γ f x y},
-      Σ ;;; Γ |- x = y ->
-      Σ ;;; Γ |- tApp f x = tApp f y.
-  Proof.
-    intros Γ f x y [h1 h2].
-  Admitted.
-
-  Lemma conv_Prod_l :
-    forall {Γ na A1 A2 B},
-      Σ ;;; Γ |- A1 = A2 ->
-      Σ ;;; Γ |- tProd na A1 B = tProd na A2 B.
-  Proof.
-  Admitted.
-
-  Lemma cumul_Prod_r :
-    forall {Γ na A B1 B2},
-      Σ ;;; Γ ,, vass na A |- B1 <= B2 ->
-      Σ ;;; Γ |- tProd na A B1 <= tProd na A B2.
-  Proof.
-    intros Γ na A B1 B2 h.
-    induction h.
-    - eapply cumul_refl. constructor.
-      + apply leq_term_refl.
-      + assumption.
-    - eapply cumul_red_l ; try eassumption.
-      econstructor. assumption.
-    - eapply cumul_red_r ; try eassumption.
-      econstructor. assumption.
-  Qed.
-
-  Lemma conv_Prod :
-    forall leq Γ na na' A1 A2 B1 B2,
-      Σ ;;; Γ |- A1 = A2 ->
-      conv leq Σ (Γ,, vass na A1) B1 B2 ->
-      conv leq Σ Γ (tProd na A1 B1) (tProd na' A2 B2).
-  Admitted.
-
-  Lemma cumul_context :
-    forall Γ u v ρ,
-      Σ ;;; Γ |- u <= v ->
-      Σ ;;; Γ |- zipc u ρ <= zipc v ρ.
-  Proof.
-    intros Γ u v ρ h.
-    revert u v h. induction ρ ; intros u v h.
-    - cbn. assumption.
-    - cbn. apply IHρ.
-      eapply cumul_App_l. assumption.
-    - cbn. eapply IHρ.
-      (* eapply conv_App_r. *)
-      (* Congruence for application on the right *)
-      admit.
-    - cbn.
-      (* Congruence for case *)
-      admit.
-  Admitted.
-
-  Lemma conv_context :
-    forall Γ u v ρ,
-      Σ ;;; Γ |- u = v ->
-      Σ ;;; Γ |- zipc u ρ = zipc v ρ.
-  Proof.
-    intros Γ u v ρ [].
-    constructor ; eapply cumul_context ; assumption.
-  Qed.
-
-  Lemma conv_context' :
-    forall Γ leq u v ρ,
-      conv leq Σ Γ u v ->
-      conv leq Σ Γ (zipc u ρ) (zipc v ρ).
-  Proof.
-    intros Γ leq u v ρ h.
-    destruct leq.
-    - cbn in *. destruct h as [[h1 h2]]. constructor.
-      constructor ; eapply cumul_context ; assumption.
-    - cbn in *. destruct h. constructor.
-      eapply cumul_context. assumption.
-  Qed.
-
-  Lemma cumul_it_mkLambda_or_LetIn :
-    forall Δ Γ u v,
-      Σ ;;; (Δ ,,, Γ) |- u <= v ->
-      Σ ;;; Δ |- it_mkLambda_or_LetIn Γ u <= it_mkLambda_or_LetIn Γ v.
-  Proof.
-    intros Δ Γ u v h. revert Δ u v h.
-    induction Γ as [| [na [b|] A] Γ ih ] ; intros Δ u v h.
-    - assumption.
-    - simpl. cbn. eapply ih.
-      (* Need cumul for LetIn *)
-      admit.
-    - simpl. cbn. eapply ih.
-      (* Need cumul for Lambda *)
-      admit.
-  Admitted.
-
-  Lemma cumul_zippx :
-    forall Γ u v ρ,
-      Σ ;;; (Γ ,,, stack_context ρ) |- u <= v ->
-      Σ ;;; Γ |- zippx u ρ <= zippx v ρ.
-  Proof.
-    intros Γ u v ρ h.
-    revert u v h. induction ρ ; intros u v h.
-    - cbn. assumption.
-    - unfold zippx. simpl.
-      case_eq (decompose_stack ρ). intros l π e.
-      unfold zippx in IHρ. rewrite e in IHρ.
-      apply IHρ.
-      eapply cumul_App_l. assumption.
-    - unfold zippx. simpl.
-      eapply cumul_it_mkLambda_or_LetIn.
-      assumption.
-    - unfold zippx. simpl.
-      eapply cumul_it_mkLambda_or_LetIn.
-      assumption.
-    - unfold zippx. simpl.
-      eapply cumul_it_mkLambda_or_LetIn.
-      assumption.
-    - unfold zippx. simpl.
-      eapply cumul_it_mkLambda_or_LetIn. cbn.
-      (* Need cumul for Lambda again *)
-      admit.
-    - unfold zippx. simpl.
-      eapply cumul_it_mkLambda_or_LetIn.
-      assumption.
-    - unfold zippx. simpl.
-      eapply cumul_it_mkLambda_or_LetIn. cbn.
-      (* cumul lambda *)
-      admit.
-  Admitted.
-
-  Lemma conv_zippx :
-    forall Γ u v ρ,
-      Σ ;;; Γ ,,, stack_context ρ |- u = v ->
-      Σ ;;; Γ |- zippx u ρ = zippx v ρ.
-  Proof.
-    intros Γ u v ρ [].
-    constructor ; eapply cumul_zippx ; assumption.
-  Qed.
-
-  Lemma conv_zippx' :
-    forall Γ leq u v ρ,
-      conv leq Σ (Γ ,,, stack_context ρ) u v ->
-      conv leq Σ Γ (zippx u ρ) (zippx v ρ).
-  Proof.
-    intros Γ leq u v ρ h.
-    destruct leq.
-    - cbn in *. destruct h as [[h1 h2]]. constructor.
-      constructor ; eapply cumul_zippx ; assumption.
-    - cbn in *. destruct h. constructor.
-      eapply cumul_zippx. assumption.
-  Qed.
 
   Inductive state :=
   | Reduction (t : term)
@@ -495,9 +65,6 @@ Section Conversion.
     intro s. destruct s ; eauto.
   Qed.
 
-  (* Notation wtp Γ t π := *)
-  (*   (welltyped Σ Γ (zippx t π)) (only parsing). *)
-
   Notation wtp Γ t π :=
     (welltyped Σ [] (zipx Γ t π)) (only parsing).
 
@@ -507,530 +74,6 @@ Section Conversion.
     | Term t' => wtp Γ t' π
     | Args => wtp Γ t π
     end.
-
-  (* TODO MOVE *)
-  Local Ltac lih :=
-    lazymatch goal with
-    | ih : forall v n k, eq_term_upto_univ _ ?u _ -> _
-      |- eq_term_upto_univ _ (lift _ _ ?u) _ =>
-      eapply ih
-    end.
-
-  Lemma eq_term_upto_univ_lift :
-    forall R u v n k,
-      eq_term_upto_univ R u v ->
-      eq_term_upto_univ R (lift n k u) (lift n k v).
-  Proof.
-    intros R u v n k e.
-    induction u in v, n, k, e |- * using term_forall_list_ind.
-    all: dependent destruction e.
-    all: try (cbn ; constructor ; try lih ; assumption).
-    - cbn. destruct (Nat.leb_spec0 k n0).
-      + constructor.
-      + constructor.
-    - cbn. constructor.
-      eapply Forall2_map.
-      eapply Forall2_impl'.
-      + eassumption.
-      + eapply All_Forall.
-        eapply All_impl ; [ eassumption |].
-        intros x H1 y H2. cbn in H1.
-        eapply H1. assumption.
-    - cbn. constructor ; try lih ; try assumption.
-      eapply Forall2_map. eapply Forall2_impl' ; [ eassumption |].
-      eapply All_Forall. eapply All_impl ; [ eassumption |].
-      intros x H0 y [? ?]. cbn in H0. repeat split ; auto.
-      eapply H0. assumption.
-    - cbn. constructor.
-      eapply Forall2_map. eapply Forall2_impl' ; [ eassumption |].
-      eapply All_Forall. eapply All_impl ; [ eassumption |].
-      intros x [h1 h2] y [? [? ?]].
-      repeat split ; auto.
-      + eapply h1. assumption.
-      + apply Forall2_length in H. rewrite H.
-        eapply h2. assumption.
-    - cbn. constructor.
-      eapply Forall2_map. eapply Forall2_impl' ; [ eassumption |].
-      eapply All_Forall. eapply All_impl ; [ eassumption |].
-      intros x [h1 h2] y [? [? ?]].
-      repeat split ; auto.
-      + eapply h1. assumption.
-      + apply Forall2_length in H. rewrite H.
-        eapply h2. assumption.
-  Qed.
-
-  (* TODO MOVE *)
-  Local Ltac sih :=
-    lazymatch goal with
-    | ih : forall v n x y, eq_term_upto_univ _ ?u _ -> _ -> _
-      |- eq_term_upto_univ _ (subst _ _ ?u) _ => eapply ih
-    end.
-
-  (* TODO MOVE *)
-  Lemma eq_term_upto_univ_subst :
-    forall R u v n x y,
-      eq_term_upto_univ R u v ->
-      eq_term_upto_univ R x y ->
-      eq_term_upto_univ R (u{n := x}) (v{n := y}).
-  Proof.
-    intros R u v n x y e1 e2.
-    induction u in v, n, x, y, e1, e2 |- * using term_forall_list_ind.
-    all: dependent destruction e1.
-    all: try (cbn ; constructor ; try sih ; assumption).
-    - cbn. destruct (Nat.leb_spec0 n n0).
-      + destruct (eqb_spec n0 n).
-        * subst. replace (n - n) with 0 by omega. cbn.
-          eapply eq_term_upto_univ_lift. assumption.
-        * replace (n0 - n) with (S (n0 - (S n))) by omega. cbn.
-          rewrite nth_error_nil. constructor.
-      + constructor.
-    - cbn. constructor.
-      eapply Forall2_map. eapply Forall2_impl' ; [ eassumption |].
-      eapply All_Forall.
-      eapply All_impl ; [ eassumption |].
-      intros x0 H1 y0 H2. cbn in H1.
-      eapply H1. all: assumption.
-    - cbn. constructor ; try sih ; try assumption.
-      eapply Forall2_map. eapply Forall2_impl' ; [ eassumption |].
-      eapply All_Forall. eapply All_impl ; [ eassumption |].
-      intros ? H0 ? [? ?]. cbn in H0. repeat split ; auto.
-      eapply H0. all: assumption.
-    - cbn. constructor.
-      eapply Forall2_map. eapply Forall2_impl' ; [ eassumption |].
-      eapply All_Forall. eapply All_impl ; [ eassumption |].
-      intros ? [h1 h2] ? [? [? ?]].
-      repeat split ; auto.
-      + eapply h1. all: assumption.
-      + apply Forall2_length in H. rewrite H.
-        eapply h2. all: assumption.
-    - cbn. constructor.
-      eapply Forall2_map. eapply Forall2_impl' ; [ eassumption |].
-      eapply All_Forall. eapply All_impl ; [ eassumption |].
-      intros ? [h1 h2] ? [? [? ?]].
-      repeat split ; auto.
-      + eapply h1. all: assumption.
-      + apply Forall2_length in H. rewrite H.
-        eapply h2. all: assumption.
-  Qed.
-
-  (* TODO MOVE *)
-  Lemma eq_term_upto_univ_mkApps_l_inv :
-    forall R u l t,
-      eq_term_upto_univ R (mkApps u l) t ->
-      exists u' l',
-        eq_term_upto_univ R u u' /\
-        Forall2 (eq_term_upto_univ R) l l' /\
-        t = mkApps u' l'.
-  Proof.
-    intros R u l t h.
-    induction l in u, t, h |- *.
-    - cbn in h. exists t, []. split ; auto.
-    - cbn in h. apply IHl in h as [u' [l' [h1 [h2 h3]]]].
-      dependent destruction h1. subst.
-      eexists. eexists. split ; [ | split ].
-      + eassumption.
-      + constructor.
-        * eassumption.
-        * eassumption.
-      + cbn. reflexivity.
-  Qed.
-
-  (* TODO MOVE *)
-  Lemma eq_term_upto_univ_mkApps :
-    forall R u1 l1 u2 l2,
-      eq_term_upto_univ R u1 u2 ->
-      Forall2 (eq_term_upto_univ R) l1 l2 ->
-      eq_term_upto_univ R (mkApps u1 l1) (mkApps u2 l2).
-  Proof.
-    intros R u1 l1 u2 l2 hu hl.
-    induction l1 in u1, u2, l2, hu, hl |- *.
-    - inversion hl. subst. assumption.
-    - inversion hl. subst. simpl.
-      eapply IHl1.
-      + constructor. all: assumption.
-      + assumption.
-  Qed.
-
-  (* TODO MOVE *)
-  Lemma Forall2_nth :
-    forall A B P l l' n (d : A) (d' : B),
-      Forall2 P l l' ->
-      P d d' ->
-      P (nth n l d) (nth n l' d').
-  Proof.
-    intros A B P l l' n d d' h hd.
-    induction n in l, l', h |- *.
-    - destruct h.
-      + assumption.
-      + assumption.
-    - destruct h.
-      + assumption.
-      + simpl. apply IHn. assumption.
-  Qed.
-
-  Arguments skipn : simpl nomatch.
-
-  (* TODO MOVE *)
-  Lemma Forall2_skipn :
-    forall A B P l l' n,
-      @Forall2 A B P l l' ->
-      Forall2 P (skipn n l) (skipn n l').
-  Proof.
-    intros A B P l l' n h.
-    induction n in l, l', h |- *.
-    - assumption.
-    - destruct h.
-      + constructor.
-      + simpl. apply IHn. assumption.
-  Qed.
-
-  Lemma Forall2_nth_error_Some_l :
-    forall A B (P : A -> B -> Prop) l l' n t,
-      nth_error l n = Some t ->
-      Forall2 P l l' ->
-      exists t',
-        nth_error l' n = Some t' /\
-        P t t'.
-  Proof.
-    intros A B P l l' n t e h.
-    induction n in l, l', t, e, h |- *.
-    - destruct h.
-      + cbn in e. discriminate.
-      + cbn in e. inversion e. subst.
-        exists y. split ; auto.
-    - destruct h.
-      + cbn in e. discriminate.
-      + cbn in e. apply IHn with (l' := l') in e ; assumption.
-  Qed.
-
-  (* TODO MOVE *)
-  Lemma eq_term_upto_univ_isApp :
-    forall R u v,
-      eq_term_upto_univ R u v ->
-      isApp u = isApp v.
-  Proof.
-    intros R u v h.
-    induction h.
-    all: reflexivity.
-  Qed.
-
-  (* TODO MOVE *)
-  Lemma isApp_mkApps :
-    forall u l,
-      isApp u ->
-      isApp (mkApps u l).
-  Proof.
-    intros u l h.
-    induction l in u, h |- *.
-    - cbn. assumption.
-    - cbn. apply IHl. reflexivity.
-  Qed.
-
-  (* TODO MOVE *)
-  Fixpoint nApp t :=
-    match t with
-    | tApp u _ => S (nApp u)
-    | _ => 0
-    end.
-
-  (* TODO MOVE *)
-  Lemma nApp_mkApps :
-    forall t l,
-      nApp (mkApps t l) = nApp t + #|l|.
-  Proof.
-    intros t l.
-    induction l in t |- *.
-    - simpl. omega.
-    - simpl. rewrite IHl. cbn. omega.
-  Qed.
-
-  (* TODO MOVE *)
-  Lemma mkApps_nApp_inj :
-    forall u u' l l',
-      nApp u = nApp u' ->
-      mkApps u l = mkApps u' l' ->
-      u = u' /\ l = l'.
-  Proof.
-    intros u u' l l' h e.
-    induction l in u, u', l', h, e |- *.
-    - cbn in e. subst.
-      destruct l' ; auto.
-      exfalso.
-      rewrite nApp_mkApps in h. cbn in h. omega.
-    - destruct l'.
-      + cbn in e. subst. exfalso.
-        rewrite nApp_mkApps in h. cbn in h. omega.
-      + cbn in e. apply IHl in e.
-        * destruct e as [e1 e2].
-          inversion e1. subst. auto.
-        * cbn. f_equal. auto.
-  Qed.
-
-  (* TODO MOVE *)
-  Lemma isApp_false_nApp :
-    forall u,
-      isApp u = false ->
-      nApp u = 0.
-  Proof.
-    intros u h.
-    destruct u.
-    all: try reflexivity.
-    discriminate.
-  Qed.
-
-  (* TODO MOVE *)
-  Lemma mkApps_notApp_inj :
-    forall u u' l l',
-      isApp u = false ->
-      isApp u' = false ->
-      mkApps u l = mkApps u' l' ->
-      u = u' /\ l = l'.
-  Proof.
-    intros u u' l l' h h' e.
-    eapply mkApps_nApp_inj.
-    - rewrite 2!isApp_false_nApp by assumption. reflexivity.
-    - assumption.
-  Qed.
-
-  (* TODO MOVE *)
-  Lemma eq_term_upto_univ_mkApps_inv :
-    forall R u l u' l',
-      isApp u = false ->
-      isApp u' = false ->
-      eq_term_upto_univ R (mkApps u l) (mkApps u' l') ->
-      eq_term_upto_univ R u u' /\ Forall2 (eq_term_upto_univ R) l l'.
-  Proof.
-    intros R u l u' l' hu hu' h.
-    apply eq_term_upto_univ_mkApps_l_inv in h as hh.
-    destruct hh as [v [args [h1 [h2 h3]]]].
-    apply eq_term_upto_univ_isApp in h1 as hh1. rewrite hu in hh1.
-    apply mkApps_notApp_inj in h3 ; auto.
-    destruct h3 as [? ?]. subst. split ; auto.
-  Qed.
-
-  (* TODO MOVE *)
-  Lemma decompose_app_rec_notApp :
-    forall t l u l',
-      decompose_app_rec t l = (u, l') ->
-      isApp u = false.
-  Proof.
-    intros t l u l' e.
-    induction t in l, u, l', e |- *.
-    all: try (cbn in e ; inversion e ; reflexivity).
-    cbn in e. eapply IHt1. eassumption.
-  Qed.
-
-  (* TODO MOVE *)
-  Lemma decompose_app_notApp :
-    forall t u l,
-      decompose_app t = (u, l) ->
-      isApp u = false.
-  Proof.
-    intros t u l e.
-    eapply decompose_app_rec_notApp. eassumption.
-  Qed.
-
-  (* TODO MOVE? *)
-  Lemma isConstruct_app_eq_term_l :
-    forall R u v,
-      isConstruct_app u ->
-      eq_term_upto_univ R u v ->
-      isConstruct_app v.
-  Proof.
-    intros R u v h e.
-    case_eq (decompose_app u). intros t1 l1 e1.
-    case_eq (decompose_app v). intros t2 l2 e2.
-    unfold isConstruct_app in *.
-    rewrite e1 in h. cbn in h.
-    rewrite e2. cbn.
-    destruct t1 ; try discriminate.
-    apply PCUICConfluence.decompose_app_inv in e1 as ?. subst.
-    apply PCUICConfluence.decompose_app_inv in e2 as ?. subst.
-    apply eq_term_upto_univ_mkApps_inv in e as hh.
-    - destruct hh as [h1 h2].
-      dependent destruction h1. reflexivity.
-    - reflexivity.
-    - eapply decompose_app_notApp. eassumption.
-  Qed.
-
-  (* TODO MOVE *)
-  (* Subsumes the other lemma? *)
-  Lemma eq_term_upto_univ_substs :
-    forall R u v n l l',
-      eq_term_upto_univ R u v ->
-      Forall2 (eq_term_upto_univ R) l l' ->
-      eq_term_upto_univ R (subst l n u) (subst l' n v).
-  Proof.
-    intros R u v n l l' hu hl.
-    induction u in v, n, l, l', hu, hl |- * using term_forall_list_ind.
-    all: dependent destruction hu.
-    all: try (cbn ; constructor ; try sih ; assumption).
-(*     - cbn. destruct (Nat.leb_spec0 n n0). *)
-(*       + destruct (eqb_spec n0 n). *)
-(*         * subst. replace (n - n) with 0 by omega. *)
-(*           destruct hl. *)
-(*           -- cbn. constructor. *)
-(*           -- cbn. eapply eq_term_upto_univ_lift. assumption. *)
-(*         * replace (n0 - n) with (S (n0 - (S n))) by omega. *)
-(*           destruct hl. *)
-(*           -- cbn. constructor. *)
-(*           -- cbn.  *)
-
-(* induction hl in n |- *. *)
-(*       + rewrite subst_empty. constructor. *)
-(*       + cbn. destruct (Nat.leb_spec0 n n0). *)
-(*         * destruct (eqb_spec n0 n). *)
-(*           -- subst. replace (n - n) with 0 by omega. cbn. *)
-(*              eapply eq_term_upto_univ_lift. assumption. *)
-(*           -- replace (n0 - n) with (S (n0 - (S n))) by omega. cbn. *)
-(*              cbn in IHhl. specialize (IHhl (S n)). *)
-(*              revert IHhl. *)
-(*              destruct (Nat.leb_spec0 (S n) n0) ; try (exfalso ; omega). *)
-(*              case_eq (nth_error l (n0 - S n)). *)
-(*              ++ intros b e. *)
-(*                 case_eq (nth_error l' (n0 - S n)). *)
-(*                 ** intros b' e' ih. *)
-
-
-
-(* cbn. destruct (Nat.leb_spec0 n n0). *)
-(*       + destruct (eqb_spec n0 n). *)
-(*         * subst. replace (n - n) with 0 by omega. *)
-(*           destruct hl. *)
-(*           -- cbn. constructor. *)
-(*           -- cbn. eapply eq_term_upto_univ_lift. assumption. *)
-(*         * replace (n0 - n) with (S (n0 - (S n))) by omega. *)
-(*           destruct hl. *)
-(*           -- cbn. constructor. *)
-(*           -- cbn. *)
-
-(*           eapply eq_term_upto_univ_lift. assumption. *)
-(*         * replace (n0 - n) with (S (n0 - (S n))) by omega. cbn. *)
-(*           rewrite nth_error_nil. constructor. *)
-(*       + constructor. *)
-    - admit.
-    - cbn. constructor.
-      eapply Forall2_map. eapply Forall2_impl' ; [ eassumption |].
-      eapply All_Forall.
-      eapply All_impl ; [ eassumption |].
-      intros x0 H1 y0 H2. cbn in H1.
-      eapply H1. all: assumption.
-    - cbn. constructor ; try sih ; try assumption.
-      eapply Forall2_map. eapply Forall2_impl' ; [ eassumption |].
-      eapply All_Forall. eapply All_impl ; [ eassumption |].
-      intros ? H0 ? [? ?]. cbn in H0. repeat split ; auto.
-      eapply H0. all: assumption.
-    - cbn. constructor.
-      eapply Forall2_map. eapply Forall2_impl' ; [ eassumption |].
-      eapply All_Forall. eapply All_impl ; [ eassumption |].
-      intros ? [h1 h2] ? [? [? ?]].
-      repeat split ; auto.
-      + eapply h1. all: assumption.
-      + apply Forall2_length in H. rewrite H.
-        eapply h2. all: assumption.
-    - cbn. constructor.
-      eapply Forall2_map. eapply Forall2_impl' ; [ eassumption |].
-      eapply All_Forall. eapply All_impl ; [ eassumption |].
-      intros ? [h1 h2] ? [? [? ?]].
-      repeat split ; auto.
-      + eapply h1. all: assumption.
-      + apply Forall2_length in H. rewrite H.
-        eapply h2. all: assumption.
-  Admitted.
-
-  (* TODO MOVE *)
-  Lemma red1_eq_term_upto_univ_l :
-    forall R Γ u v u',
-      Reflexive R ->
-      eq_term_upto_univ R u u' ->
-      red1 Σ Γ u v ->
-      exists v',
-        ∥ red1 Σ Γ u' v' ∥ /\
-        eq_term_upto_univ R v v'.
-  Proof.
-    intros R Γ u v u' hR e h.
-    induction h in u', e |- *.
-    - dependent destruction e. dependent destruction e1.
-      eexists. split.
-      + constructor. constructor.
-      + eapply eq_term_upto_univ_subst ; assumption.
-    - dependent destruction e.
-      eexists. split.
-      + constructor. constructor.
-      + eapply eq_term_upto_univ_subst ; assumption.
-    - dependent destruction e.
-      eexists. split.
-      + constructor. constructor. eassumption.
-      + eapply eq_term_upto_univ_refl. assumption.
-    - dependent destruction e.
-      apply eq_term_upto_univ_mkApps_l_inv in e2 as [? [? [h1 [h2 h3]]]]. subst.
-      dependent destruction h1.
-      eexists. split.
-      + constructor. constructor.
-      + eapply eq_term_upto_univ_mkApps.
-        * eapply Forall2_nth with (P := fun x y => eq_term_upto_univ R (snd x) (snd y)).
-          -- eapply Forall2_impl ; [ eassumption |].
-             intros x y [? ?]. assumption.
-          -- cbn. eapply eq_term_upto_univ_refl. assumption.
-        * eapply Forall2_skipn. assumption.
-    - apply eq_term_upto_univ_mkApps_l_inv in e as [? [? [h1 [h2 h3]]]]. subst.
-      dependent destruction h1.
-      unfold unfold_fix in e0.
-      case_eq (nth_error mfix idx) ;
-        try (intros e ; rewrite e in e0 ; discriminate e0).
-      intros d e. rewrite e in e0. inversion e0. subst. clear e0.
-      eapply Forall2_nth_error_Some_l in H as hh ; try eassumption.
-      destruct hh as [d' [e' [? [? erarg]]]].
-      unfold is_constructor in e1.
-      case_eq (nth_error args (rarg d)) ;
-        try (intros bot ; rewrite bot in e1 ; discriminate e1).
-      intros a ea. rewrite ea in e1.
-      eapply Forall2_nth_error_Some_l in h2 as hh ; try eassumption.
-      destruct hh as [a' [ea' ?]].
-      eexists. split.
-      + constructor. eapply red_fix.
-        * unfold unfold_fix. rewrite e'. reflexivity.
-        * unfold is_constructor. rewrite <- erarg. rewrite ea'.
-          eapply isConstruct_app_eq_term_l ; eassumption.
-      + eapply eq_term_upto_univ_mkApps.
-        * eapply eq_term_upto_univ_substs.
-          -- assumption.
-          --
-  Admitted.
-
-  Lemma cored_eq_term_upto_univ_r :
-    forall R Γ u v u',
-      Reflexive R ->
-      eq_term_upto_univ R u u' ->
-      cored Σ Γ v u ->
-      exists v',
-        cored Σ Γ v' u' /\
-        eq_term_upto_univ R v v'.
-  Proof.
-    intros R Γ u v u' hR e h.
-    induction h.
-    - eapply red1_eq_term_upto_univ_l in X ; try eassumption.
-      destruct X as [v' [[r] e']].
-      exists v'. split ; auto.
-      constructor. assumption.
-    - specialize (IHh e). destruct IHh as [v' [c ev]].
-      eapply red1_eq_term_upto_univ_l in X ; try eassumption.
-      destruct X as [w' [[?] ?]].
-      exists w'. split ; auto.
-      eapply cored_trans ; eauto.
-  Qed.
-
-  Lemma cored_nl :
-    forall Γ u v,
-      cored Σ Γ u v ->
-      cored Σ (nlctx Γ) (nl u) (nl v).
-  Admitted.
-
-  Lemma red_nl :
-    forall Γ u v,
-      red Σ Γ u v ->
-      red Σ (nlctx Γ) (nl u) (nl v).
-  Admitted.
 
   Set Primitive Projections.
 
@@ -1054,105 +97,6 @@ Section Conversion.
     | Args => Args
     end.
 
-  Fixpoint nlstack (π : stack) : stack :=
-    match π with
-    | ε => ε
-
-    | App u ρ =>
-      App (nl u) (nlstack ρ)
-
-    | Fix f n args ρ =>
-      Fix (map (map_def_anon nl nl) f) n (map nl args) (nlstack ρ)
-
-    | Case indn p brs ρ =>
-      Case indn (nl p) (map (on_snd nl) brs) (nlstack ρ)
-
-    | Prod_l na B ρ =>
-      Prod_l nAnon (nl B) (nlstack ρ)
-
-    | Prod_r na A ρ =>
-      Prod_r nAnon (nl A) (nlstack ρ)
-
-    | Lambda_ty na b ρ =>
-      Lambda_ty nAnon (nl b) (nlstack ρ)
-
-    | Lambda_tm na A ρ =>
-      Lambda_tm nAnon (nl A) (nlstack ρ)
-
-    | coApp t ρ =>
-      coApp (nl t) (nlstack ρ)
-    end.
-
-  Lemma nlstack_appstack :
-    forall args ρ,
-      nlstack (appstack args ρ) = appstack (map nl args) (nlstack ρ).
-  Proof.
-    intros args ρ.
-    induction args in ρ |- *.
-    - reflexivity.
-    - simpl. f_equal. eapply IHargs.
-  Qed.
-
-  Lemma nlstack_cat :
-    forall ρ θ,
-      nlstack (ρ +++ θ) = nlstack ρ +++ nlstack θ.
-  Proof.
-    intros ρ θ.
-    induction ρ in θ |- *.
-    all: solve [ simpl ; rewrite ?IHρ ; reflexivity ].
-  Qed.
-
-  Lemma stack_position_nlstack :
-    forall ρ,
-      stack_position (nlstack ρ) = stack_position ρ.
-  Proof.
-    intros ρ.
-    induction ρ.
-    all: (simpl ; rewrite ?IHρ ; reflexivity).
-  Qed.
-
-  Lemma nl_it_mkLambda_or_LetIn :
-    forall Γ t,
-      nl (it_mkLambda_or_LetIn Γ t) =
-      it_mkLambda_or_LetIn (nlctx Γ) (nl t).
-  Proof.
-    intros Γ t.
-    induction Γ as [| [na [b|] B] Γ ih] in t |- *.
-    - reflexivity.
-    - simpl. cbn. rewrite ih. reflexivity.
-    - simpl. cbn. rewrite ih. reflexivity.
-  Qed.
-
-  Lemma nl_mkApps :
-    forall t l,
-      nl (mkApps t l) = mkApps (nl t) (map nl l).
-  Proof.
-    intros t l.
-    induction l in t |- *.
-    - reflexivity.
-    - simpl. rewrite IHl. reflexivity.
-  Qed.
-
-  Lemma nl_zipc :
-    forall t π,
-      nl (zipc t π) = zipc (nl t) (nlstack π).
-  Proof.
-    intros t π.
-    induction π in t |- *.
-    all: try solve [ simpl ; rewrite ?IHπ ; reflexivity ].
-    simpl. rewrite IHπ. cbn. f_equal.
-    rewrite nl_mkApps. reflexivity.
-  Qed.
-
-  Lemma nl_zipx :
-    forall Γ t π,
-      nl (zipx Γ t π) = zipx (nlctx Γ) (nl t) (nlstack π).
-  Proof.
-    intros Γ t π.
-    unfold zipx. rewrite nl_it_mkLambda_or_LetIn. f_equal.
-    apply nl_zipc.
-  Qed.
-
   Lemma nl_wth :
     forall {Γ s t π2},
       let t' :=
@@ -1171,7 +115,7 @@ Section Conversion.
       welltyped Σ [] (zipx (nlctx Γ) nlt' (nlstack π2)).
   Proof.
     intros Γ s t π2 t' nlt' h.
-    eapply welltyped_rename.
+    eapply welltyped_rename ; try assumption.
     - exact h.
     - destruct s.
       + cbn in nlt'.
@@ -1185,25 +129,10 @@ Section Conversion.
         eapply eq_term_tm_nl.
   Qed.
 
-  Lemma nlctx_app_context :
-    forall Γ Δ,
-      nlctx (Γ ,,, Δ) = nlctx Γ ,,, nlctx Δ.
-  Proof.
-    intros Γ Δ.
-    induction Δ as [| [na [b|] B] Δ ih] in Γ |- *.
-    - reflexivity.
-    - simpl. f_equal. apply ih.
-    - simpl. f_equal. apply ih.
-  Qed.
-
-  Lemma nlctx_stack_context :
-    forall ρ,
-      nlctx (stack_context ρ) = stack_context (nlstack ρ).
-  Proof.
-    intro ρ. induction ρ.
-    all: (simpl ; rewrite ?IHρ ; reflexivity).
-  Qed.
-
+  (* TODO Maybe have a type of pack and an R that already operates on namless
+     stuff.
+     Then have R x y defined as "R_nl (nl x) (nl y)".
+   *)
   Definition nlmkpack s Γ t π1 π2 h :=
     mkpack (nlstate s) (nlctx Γ) (nl t) (nlstack π1) (nlstack π2) (nl_wth h).
 
@@ -1252,29 +181,6 @@ Section Conversion.
           -- intro. eapply stateR_Acc.
         * eapply wcored_wf.
     - eapply normalisation. eassumption.
-  Qed.
-
-  Lemma wf_fun :
-    forall A (R : A -> A -> Prop) B (f : B -> A),
-      well_founded R ->
-      well_founded (fun x y => R (f x) (f y)).
-  Proof.
-    intros A R B f h x.
-    specialize (h (f x)).
-    dependent induction h.
-    constructor. intros y h.
-    eapply H0 ; try reflexivity. assumption.
-  Qed.
-
-  Lemma Acc_fun :
-    forall A (R : A -> A -> Prop) B (f : B -> A) x,
-      Acc R (f x) ->
-      Acc (fun x y => R (f x) (f y)) x.
-  Proof.
-    intros A R B f x h.
-    dependent induction h.
-    constructor. intros y h.
-    eapply H0 ; try reflexivity. assumption.
   Qed.
 
   Lemma R_Acc :
@@ -1349,159 +255,6 @@ Section Conversion.
     right. right. right. right. assumption.
   Qed.
 
-  Lemma inversion_LetIn :
-    forall {Γ na b B t T},
-      Σ ;;; Γ |- tLetIn na b B t : T ->
-      exists s1 A,
-        ∥ Σ ;;; Γ |- B : tSort s1 ∥ /\
-        ∥ Σ ;;; Γ |- b : B ∥ /\
-        ∥ Σ ;;; Γ ,, vdef na b B |- t : A ∥ /\
-        ∥ Σ ;;; Γ |- tLetIn na b B A <= T ∥.
-  Proof.
-    intros Γ na b B t T h. dependent induction h.
-    - exists s1, b'_ty. split ; [| split ; [| split]].
-      + constructor. assumption.
-      + constructor. assumption.
-      + constructor. assumption.
-      + constructor. apply cumul_refl'.
-    - destruct IHh as [s1 [A' [? [? [? hc]]]]].
-      exists s1, A'. split ; [| split ; [| split]].
-      all: try assumption.
-      destruct hc.
-      constructor. eapply cumul_trans ; eassumption.
-  Qed.
-
-  Lemma welltyped_it_mkLambda_or_LetIn :
-    forall Γ Δ t,
-      welltyped Σ Γ (it_mkLambda_or_LetIn Δ t) ->
-      welltyped Σ (Γ ,,, Δ) t.
-  Proof.
-    intros Γ Δ t h.
-    revert Γ t h.
-    induction Δ as [| [na [b|] A] Δ ih ] ; intros Γ t h.
-    - assumption.
-    - simpl. apply ih in h. cbn in h.
-      destruct h as [T h].
-      pose proof (inversion_LetIn h) as [s1 [A' [[?] [[?] [[?] [?]]]]]].
-      exists A'. assumption.
-    - simpl. apply ih in h. cbn in h.
-      destruct h as [T h].
-      pose proof (inversion_Lambda h) as [s1 [B [[?] [[?] [?]]]]].
-      exists B. assumption.
-  Qed.
-
-  Lemma welltyped_zipp :
-    forall Γ t ρ,
-      welltyped Σ Γ (zipp t ρ) ->
-      welltyped Σ Γ t.
-  Proof.
-    intros Γ t ρ [A h].
-    unfold zipp in h.
-    case_eq (decompose_stack ρ). intros l π e.
-    rewrite e in h. clear - h.
-    revert t A h.
-    induction l ; intros t A h.
-    - eexists. cbn in h. eassumption.
-    - cbn in h. apply IHl in h.
-      destruct h as [T h].
-      destruct (inversion_App h) as [na [A' [B' [[?] [[?] [?]]]]]].
-      eexists. eassumption.
-  Qed.
-
-  Lemma welltyped_zippx :
-    forall Γ t ρ,
-      welltyped Σ Γ (zippx t ρ) ->
-      welltyped Σ (Γ ,,, stack_context ρ) t.
-  Proof.
-    intros Γ t ρ h.
-    unfold zippx in h.
-    case_eq (decompose_stack ρ). intros l π e.
-    rewrite e in h.
-    apply welltyped_it_mkLambda_or_LetIn in h.
-    pose proof (decompose_stack_eq _ _ _ e). subst.
-    rewrite stack_context_appstack.
-    clear - h. destruct h as [A h].
-    revert t A h.
-    induction l ; intros t A h.
-    - eexists. eassumption.
-    - cbn in h. apply IHl in h.
-      destruct h as [B h].
-      destruct (inversion_App h) as [na [A' [B' [[?] [[?] [?]]]]]].
-      eexists. eassumption.
-  Qed.
-
-  Derive NoConfusion NoConfusionHom for list.
-
-  Lemma it_mkLambda_or_LetIn_welltyped :
-    forall Γ Δ t,
-      welltyped Σ (Γ ,,, Δ) t ->
-      welltyped Σ Γ (it_mkLambda_or_LetIn Δ t).
-  Proof.
-    intros Γ Δ t h.
-    revert Γ t h.
-    induction Δ as [| [na [b|] B] Δ ih ] ; intros Γ t h.
-    - assumption.
-    - simpl. eapply ih. cbn.
-      destruct h as [A h].
-      pose proof (typing_wf_local h) as hc.
-      cbn in hc. dependent destruction hc.
-      + cbn in H. inversion H.
-      + cbn in H. symmetry in H. inversion H. subst. clear H.
-        cbn in l.
-        eexists. econstructor ; try eassumption.
-        (* FIXME We need to sort B, but we only know it's a type.
-           It might be a problem with the way context are wellformed.
-           Let typing asks for the type to be sorted so it should
-           also hold in the context.
-           At least they should be synchronised.
-         *)
-        admit.
-    - simpl. eapply ih. cbn.
-      destruct h as [A h].
-      pose proof (typing_wf_local h) as hc.
-      cbn in hc. dependent destruction hc.
-      + cbn in H. symmetry in H. inversion H. subst. clear H.
-        destruct l as [s hs].
-        eexists. econstructor ; eassumption.
-      + cbn in H. inversion H.
-  Admitted.
-
-  Lemma zipx_welltyped :
-    forall {Γ t π},
-      welltyped Σ Γ (zipc t π) ->
-      welltyped Σ [] (zipx Γ t π).
-  Proof.
-    intros Γ t π h.
-    eapply it_mkLambda_or_LetIn_welltyped.
-    rewrite app_context_nil_l.
-    assumption.
-  Qed.
-
-  Lemma welltyped_zipx :
-    forall {Γ t π},
-      welltyped Σ [] (zipx Γ t π) ->
-      welltyped Σ Γ (zipc t π).
-  Proof.
-    intros Γ t π h.
-    apply welltyped_it_mkLambda_or_LetIn in h.
-    rewrite app_context_nil_l in h.
-    assumption.
-  Qed.
-
-  Lemma welltyped_zipc_zippx :
-    forall Γ t π,
-      welltyped Σ Γ (zipc t π) ->
-      welltyped Σ Γ (zippx t π).
-  Proof.
-    intros Γ t π h.
-    unfold zippx.
-    case_eq (decompose_stack π). intros l ρ e.
-    pose proof (decompose_stack_eq _ _ _ e). subst.
-    eapply it_mkLambda_or_LetIn_welltyped.
-    rewrite zipc_appstack in h. zip fold in h.
-    apply welltyped_context in h. assumption.
-  Qed.
-
   Lemma zwts :
     forall {Γ s t π},
       wts Γ s t π ->
@@ -1571,7 +324,7 @@ Section Conversion.
     }.
   Next Obligation.
     apply welltyped_zipx in h1.
-    apply welltyped_zipc_zippx in h1.
+    apply welltyped_zipc_zippx in h1 ; try assumption.
     cbn. rewrite zipc_appstack. cbn.
     unfold zippx in h1. rewrite <- e1 in h1.
     apply welltyped_it_mkLambda_or_LetIn in h1.
@@ -1581,7 +334,7 @@ Section Conversion.
   Next Obligation.
     clear aux eq1.
     apply welltyped_zipx in h2.
-    apply welltyped_zipc_zippx in h2.
+    apply welltyped_zipc_zippx in h2 ; try assumption.
     cbn. rewrite zipc_appstack. cbn.
     unfold zippx in h2. rewrite <- e2 in h2.
     apply welltyped_it_mkLambda_or_LetIn in h2.
@@ -1609,13 +362,13 @@ Section Conversion.
     rewrite decompose_stack_appstack in d1. cbn in d1. subst.
     pose proof (decompose_stack_eq _ _ _ e1'). subst.
     rewrite stack_cat_appstack.
-    eapply zipx_welltyped.
+    eapply zipx_welltyped ; try assumption.
     rewrite zipc_appstack.
 
     rewrite stack_context_appstack in r1. cbn in r1.
     rewrite 2!zipc_appstack in r1. cbn in r1.
 
-    eapply red_welltyped ; revgoals.
+    eapply red_welltyped ; try assumption ; revgoals.
     - constructor. zip fold. eapply red_context. eassumption.
     - cbn. assumption.
   Qed.
@@ -1640,13 +393,13 @@ Section Conversion.
     rewrite decompose_stack_appstack in d2. cbn in d2. subst.
     pose proof (decompose_stack_eq _ _ _ e2'). subst.
     rewrite stack_cat_appstack.
-    eapply zipx_welltyped.
+    eapply zipx_welltyped ; try assumption.
     rewrite zipc_appstack.
 
     rewrite stack_context_appstack in r2. cbn in r2.
     rewrite 2!zipc_appstack in r2. cbn in r2.
 
-    eapply red_welltyped ; revgoals.
+    eapply red_welltyped ; try assumption ; revgoals.
     - constructor. zip fold. eapply red_context. eassumption.
     - cbn. assumption.
   Qed.
@@ -1698,7 +451,8 @@ Section Conversion.
              rewrite nlstack_appstack. rewrite nlstack_cat.
              rewrite zipc_appstack. rewrite zipc_stack_cat.
              repeat zip fold. eapply cored_context.
-             apply cored_nl in H. rewrite nlctx_app_context in H.
+             apply cored_nl in H ; try assumption.
+             rewrite nlctx_app_context in H.
              rewrite nlctx_stack_context in H.
              rewrite nl_zipc in H. rewrite nl_mkApps in H.
              assumption.
@@ -1732,7 +486,7 @@ Section Conversion.
         rewrite nlstack_cat. rewrite nlstack_appstack.
         rewrite zipc_appstack. rewrite zipc_stack_cat.
         repeat zip fold. eapply cored_context.
-        apply cored_nl in H. rewrite nlctx_app_context in H.
+        apply cored_nl in H ; try assumption. rewrite nlctx_app_context in H.
         rewrite nlctx_stack_context in H. rewrite nl_zipc in H.
         rewrite nl_mkApps in H.
         assumption.
@@ -1858,65 +612,6 @@ Section Conversion.
         assumption.
   Qed.
 
-  Lemma lookup_env_const_name :
-    forall {c c' d},
-      lookup_env Σ c' = Some (ConstantDecl c d) ->
-      c' = c.
-  Proof.
-    intros c c' d e. clear hΣ.
-    destruct Σ as [Σ' ?]. cbn in e.
-    induction Σ'.
-    - cbn in e. discriminate.
-    - destruct a.
-      + cbn in e. destruct (ident_eq_spec c' k).
-        * subst. inversion e. reflexivity.
-        * apply IHΣ'. assumption.
-      + cbn in e. destruct (ident_eq_spec c' k).
-        * inversion e.
-        * apply IHΣ'. assumption.
-  Qed.
-
-  Lemma red_const :
-    forall {Γ n c u cty cb cu},
-      Some (ConstantDecl n {| cst_type := cty ; cst_body := Some cb ; cst_universes := cu |})
-      = lookup_env Σ c ->
-      red (fst Σ) Γ (tConst c u) (subst_instance_constr u cb).
-  Proof.
-    intros Γ n c u cty cb cu e.
-    symmetry in e.
-    pose proof (lookup_env_const_name e). subst.
-    econstructor.
-    - econstructor.
-    - econstructor.
-      + exact e.
-      + reflexivity.
-  Qed.
-
-  Lemma cored_const :
-    forall {Γ n c u cty cb cu},
-      Some (ConstantDecl n {| cst_type := cty ; cst_body := Some cb ; cst_universes := cu |})
-      = lookup_env Σ c ->
-      cored (fst Σ) Γ (subst_instance_constr u cb) (tConst c u).
-  Proof.
-    intros Γ n c u cty cb cu e.
-    symmetry in e.
-    pose proof (lookup_env_const_name e). subst.
-    econstructor.
-    econstructor.
-    - exact e.
-    - reflexivity.
-  Qed.
-
-  Derive Signature for cumul.
-  Derive Signature for red1.
-
-  Lemma context_conversion :
-    forall {Γ t T Γ'},
-      Σ ;;; Γ |- t : T ->
-      PCUICSR.conv_context Σ Γ Γ' ->
-      Σ ;;; Γ' |- t : T.
-  Admitted.
-
   Equations unfold_one_fix (Γ : context) (mfix : mfixpoint term)
             (idx : nat) (π : stack) (h : wtp Γ (tFix mfix idx) π)
     : option (term * stack) :=
@@ -1944,32 +639,6 @@ Section Conversion.
   Qed.
 
   Derive NoConfusion NoConfusionHom for option.
-
-  Lemma app_reds_r :
-    forall Γ u v1 v2,
-      red Σ Γ v1 v2 ->
-      red Σ Γ (tApp u v1) (tApp u v2).
-  Proof.
-    intros Γ u v1 v2 h.
-    revert u. induction h ; intros u.
-    - constructor.
-    - econstructor.
-      + eapply IHh.
-      + constructor. assumption.
-  Qed.
-
-  Lemma app_cored_r :
-    forall Γ u v1 v2,
-      cored Σ Γ v1 v2 ->
-      cored Σ Γ (tApp u v1) (tApp u v2).
-  Proof.
-    intros Γ u v1 v2 h.
-    induction h.
-    - constructor. constructor. assumption.
-    - eapply cored_trans.
-      + eapply IHh.
-      + constructor. assumption.
-  Qed.
 
   Lemma unfold_one_fix_red_zippx :
     forall Γ mfix idx π h fn ξ,
@@ -2122,193 +791,6 @@ Section Conversion.
     reflexivity.
   Qed.
 
-  Lemma cored_red_cored :
-    forall Γ u v w,
-      cored Σ Γ w v ->
-      red Σ Γ u v ->
-      cored Σ Γ w u.
-  Proof.
-    intros Γ u v w h1 h2.
-    revert u h2. induction h1 ; intros t h2.
-    - eapply cored_red_trans ; eassumption.
-    - eapply cored_trans.
-      + eapply IHh1. assumption.
-      + assumption.
-  Qed.
-
-  Lemma red_cored_cored :
-    forall Γ u v w,
-      red Σ Γ v w ->
-      cored Σ Γ v u ->
-      cored Σ Γ w u.
-  Proof.
-    intros Γ u v w h1 h2.
-    revert u h2. induction h1 ; intros t h2.
-    - assumption.
-    - eapply cored_trans.
-      + eapply IHh1. assumption.
-      + assumption.
-  Qed.
-
-  Fixpoint isAppProd (t : term) : bool :=
-    match t with
-    | tApp t l => isAppProd t
-    | tProd na A B => true
-    | _ => false
-    end.
-
-  Fixpoint isProd t :=
-    match t with
-    | tProd na A B => true
-    | _ => false
-    end.
-
-  Lemma isAppProd_isProd :
-    forall Γ t,
-      isAppProd t ->
-      welltyped Σ Γ t ->
-      isProd t.
-  Proof.
-    intros Γ t hp hw.
-    revert Γ hp hw.
-    induction t ; intros Γ hp hw.
-    all: try discriminate hp.
-    - reflexivity.
-    - simpl in hp.
-      specialize IHt1 with (1 := hp).
-      assert (welltyped Σ Γ t1) as h.
-      { destruct hw as [T h].
-        destruct (inversion_App h) as [na [A' [B' [[?] [[?] [?]]]]]].
-        eexists. eassumption.
-      }
-      specialize IHt1 with (1 := h).
-      destruct t1.
-      all: try discriminate IHt1.
-      destruct hw as [T hw'].
-      destruct (inversion_App hw') as [na [A' [B' [[hP] [[?] [?]]]]]].
-      destruct (inversion_Prod hP) as [s1 [s2 [[?] [[?] [bot]]]]].
-      (* dependent destruction bot. *)
-      (* + discriminate e. *)
-      (* + dependent destruction r. *)
-      admit.
-  Admitted.
-
-  Lemma isAppProd_mkApps :
-    forall t l, isAppProd (mkApps t l) = isAppProd t.
-  Proof.
-    intros t l. revert t.
-    induction l ; intros t.
-    - reflexivity.
-    - cbn. rewrite IHl. reflexivity.
-  Qed.
-
-  Lemma isProdmkApps :
-    forall t l,
-      isProd (mkApps t l) ->
-      l = [].
-  Proof.
-    intros t l h.
-    revert t h.
-    induction l ; intros t h.
-    - reflexivity.
-    - cbn in h. specialize IHl with (1 := h). subst.
-      cbn in h. discriminate h.
-  Qed.
-
-  Lemma mkApps_Prod_nil :
-    forall Γ na A B l,
-      welltyped Σ Γ (mkApps (tProd na A B) l) ->
-      l = [].
-  Proof.
-    intros Γ na A B l h.
-    pose proof (isAppProd_isProd) as hh.
-    specialize hh with (2 := h).
-    rewrite isAppProd_mkApps in hh.
-    specialize hh with (1 := eq_refl).
-    apply isProdmkApps in hh. assumption.
-  Qed.
-
-  Lemma eq_term_it_mkLambda_or_LetIn_inv :
-    forall Γ u v,
-      eq_term (snd Σ) (it_mkLambda_or_LetIn Γ u) (it_mkLambda_or_LetIn Γ v) ->
-      eq_term (snd Σ) u v.
-  Proof.
-    intros Γ.
-    induction Γ as [| [na [b|] A] Γ ih ] ; intros u v h.
-    - assumption.
-    - simpl in h. cbn in h. apply ih in h. inversion h. subst.
-      assumption.
-    - simpl in h. cbn in h. apply ih in h. inversion h. subst.
-      assumption.
-  Qed.
-
-  Lemma eq_term_zipc_inv :
-    forall u v π,
-      eq_term (snd Σ) (zipc u π) (zipc v π) ->
-      eq_term (snd Σ) u v.
-  Proof.
-    intros u v π h.
-    revert u v h. induction π ; intros u v h.
-    all: solve [
-      simpl in h ; try apply IHπ in h ;
-      cbn in h ; inversion h ; subst ; assumption
-    ].
-  Qed.
-
-  Lemma eq_term_zipx_inv :
-    forall Γ u v π,
-      eq_term (snd Σ) (zipx Γ u π) (zipx Γ v π) ->
-      eq_term (snd Σ) u v.
-  Proof.
-    intros Γ u v π h.
-    eapply eq_term_zipc_inv.
-    eapply eq_term_it_mkLambda_or_LetIn_inv.
-    eassumption.
-  Qed.
-
-  Lemma eq_term_it_mkLambda_or_LetIn :
-    forall Γ u v,
-      eq_term (snd Σ) u v ->
-      eq_term (snd Σ) (it_mkLambda_or_LetIn Γ u) (it_mkLambda_or_LetIn Γ v).
-  Proof.
-    intros Γ.
-    induction Γ as [| [na [b|] A] Γ ih ] ; intros u v h.
-    - assumption.
-    - simpl. cbn. apply ih. constructor ; try apply eq_term_refl. assumption.
-    - simpl. cbn. apply ih. constructor ; try apply eq_term_refl. assumption.
-  Qed.
-
-  Lemma eq_term_zipc :
-    forall u v π,
-      eq_term (snd Σ) u v ->
-      eq_term (snd Σ) (zipc u π) (zipc v π).
-  Proof.
-    intros u v π h.
-    revert u v h. induction π ; intros u v h.
-    all: try solve [
-      simpl ; try apply IHπ ;
-      cbn ; constructor ; try apply eq_term_refl ; assumption
-    ].
-    - assumption.
-    - simpl. apply IHπ. destruct indn as [i n].
-      constructor.
-      + apply eq_term_refl.
-      + assumption.
-      + eapply Forall_Forall2. eapply Forall_True.
-        intros. split ; auto. apply eq_term_refl.
-  Qed.
-
-  Lemma eq_term_zipx :
-    forall Γ u v π,
-      eq_term (snd Σ) u v ->
-      eq_term (snd Σ) (zipx Γ u π) (zipx Γ v π).
-  Proof.
-    intros Γ u v π h.
-    eapply eq_term_it_mkLambda_or_LetIn.
-    eapply eq_term_zipc.
-    eassumption.
-  Qed.
-
   (* This corresponds to a subgoal I don't know how to prove, hence the ax
      suffix. *)
   Lemma conv_Prod_ax :
@@ -2319,66 +801,6 @@ Section Conversion.
      conv leq Σ Γ (it_mkLambda_or_LetIn (stack_context ρ1) (tProd na1 A1 B1))
           (it_mkLambda_or_LetIn (stack_context ρ2) (tProd na2 A2 B2)).
   Admitted.
-
-  (* TODO MOVE or even replace old lemma *)
-  Lemma decompose_stack_noStackApp :
-    forall π l ρ,
-      decompose_stack π = (l,ρ) ->
-      isStackApp ρ = false.
-  Proof.
-    intros π l ρ e.
-    destruct ρ. all: auto.
-    exfalso. eapply decompose_stack_not_app. eassumption.
-  Qed.
-
-  (* TODO MOVE *)
-  Lemma stack_context_decompose :
-    forall π,
-      stack_context (snd (decompose_stack π)) = stack_context π.
-  Proof.
-    intros π.
-    case_eq (decompose_stack π). intros l ρ e.
-    cbn. pose proof (decompose_stack_eq _ _ _ e). subst.
-    rewrite stack_context_appstack. reflexivity.
-  Qed.
-
-  Lemma eq_term_trans :
-    forall G u v w,
-      eq_term G u v ->
-      eq_term G v w ->
-      eq_term G u w.
-  Admitted.
-
-  Lemma nl_subst_instance_constr :
-    forall u b,
-      nl (subst_instance_constr u b) = subst_instance_constr u (nl b).
-  Proof.
-    intros u b.
-    induction b using term_forall_list_ind.
-    all: try (simpl ; rewrite ?IHb, ?IHb1, ?IHb2, ?IHb3 ; reflexivity).
-    - simpl. f_equal. induction H.
-      + reflexivity.
-      + simpl. rewrite p, IHAll. reflexivity.
-    - simpl. rewrite IHb1, IHb2. f_equal.
-      induction X.
-      + reflexivity.
-      + simpl. f_equal.
-        * unfold on_snd. destruct p, x. simpl in *.
-          rewrite p0. reflexivity.
-        * apply IHX.
-    - simpl. f_equal. induction X ; try reflexivity.
-      simpl. rewrite IHX. f_equal.
-      destruct p as [h1 h2].
-      destruct x. simpl in *.
-      unfold map_def, map_def_anon. cbn.
-      rewrite h1, h2. reflexivity.
-    - simpl. f_equal. induction X ; try reflexivity.
-      simpl. rewrite IHX. f_equal.
-      destruct p as [h1 h2].
-      destruct x. simpl in *.
-      unfold map_def, map_def_anon. cbn.
-      rewrite h1, h2. reflexivity.
-  Qed.
 
   Equations(noeqns) _isconv_prog (Γ : context) (leq : conv_pb)
             (t1 : term) (π1 : stack) (h1 : wtp Γ t1 π1)
@@ -2538,21 +960,21 @@ Section Conversion.
     rewrite 2!stack_context_appstack in h.
 
     apply welltyped_zipx in h1.
-    apply welltyped_zipc_zippx in h1.
+    apply welltyped_zipc_zippx in h1 ; auto.
     unfold zippx in h1. rewrite decompose_stack_appstack in h1.
     rewrite decompose_stack_twice with (1 := e1) in h1.
     simpl in h1. rewrite app_nil_r in h1.
     apply welltyped_it_mkLambda_or_LetIn in h1.
-    apply mkApps_Prod_nil in h1. subst.
+    apply mkApps_Prod_nil in h1 ; auto. subst.
 
     clear aux.
     apply welltyped_zipx in h2.
-    apply welltyped_zipc_zippx in h2.
+    apply welltyped_zipc_zippx in h2 ; auto.
     unfold zippx in h2. rewrite decompose_stack_appstack in h2.
     rewrite decompose_stack_twice with (1 := e2) in h2.
     simpl in h2. rewrite app_nil_r in h2.
     apply welltyped_it_mkLambda_or_LetIn in h2.
-    apply mkApps_Prod_nil in h2. subst.
+    apply mkApps_Prod_nil in h2 ; auto. subst.
 
     cbn.
     eapply conv_Prod_ax ; assumption.
@@ -2615,12 +1037,12 @@ Section Conversion.
     destruct h. eapply conv_conv_l. assumption.
   Qed.
   Next Obligation.
-    eapply red_welltyped.
+    eapply red_welltyped ; auto.
     - exact h1.
     - constructor. eapply red_zipx. eapply red_const. eassumption.
   Qed.
   Next Obligation.
-    eapply red_welltyped.
+    eapply red_welltyped ; auto.
     - exact h2.
     - constructor. eapply red_zipx. eapply red_const. eassumption.
   Qed.
@@ -2631,7 +1053,7 @@ Section Conversion.
     (* TODO!! Perhaps cored_nl is not true after all... *)
     change (tConst c' u') with (nl (tConst c' u')).
     rewrite <- nlctx_stack_context. rewrite <- nlctx_app_context.
-    eapply cored_nl.
+    eapply cored_nl ; auto.
     eapply cored_const.
     eassumption.
   Qed.
@@ -2647,7 +1069,7 @@ Section Conversion.
       eapply red_const. eassumption.
   Qed.
   Next Obligation.
-    eapply red_welltyped ; [ exact h2 | ].
+    eapply red_welltyped ; auto ; [ exact h2 | ].
     constructor. eapply red_zipx. eapply red_const. eassumption.
   Qed.
   Next Obligation.
@@ -2656,7 +1078,7 @@ Section Conversion.
     simpl. eapply cored_zipx.
     change (tConst c' u') with (nl (tConst c' u')).
     rewrite <- nlctx_stack_context. rewrite <- nlctx_app_context.
-    eapply cored_nl.
+    eapply cored_nl ; auto.
     eapply cored_const. eassumption.
   Qed.
   Next Obligation.
@@ -2666,14 +1088,14 @@ Section Conversion.
     eapply red_zippx. eapply red_const. eassumption.
   Qed.
   Next Obligation.
-    eapply red_welltyped ; [ exact h1 | ].
+    eapply red_welltyped ; auto ; [ exact h1 | ].
     constructor. eapply red_zipx. eapply red_const. eassumption.
   Qed.
   Next Obligation.
     left. simpl. eapply cored_zipx.
     rewrite <- nlctx_stack_context. rewrite <- nlctx_app_context.
     change (tConst c' u) with (nl (tConst c' u)).
-    eapply cored_nl.
+    eapply cored_nl ; auto.
     eapply cored_const. eassumption.
   Qed.
   Next Obligation.
@@ -2683,14 +1105,14 @@ Section Conversion.
     eapply red_zippx. eapply red_const. eassumption.
   Qed.
   Next Obligation.
-    eapply red_welltyped ; [ exact h1 | ].
+    eapply red_welltyped ; auto ; [ exact h1 | ].
     constructor. eapply red_zipx. eapply red_const. eassumption.
   Qed.
   Next Obligation.
     left. simpl. eapply cored_zipx.
     rewrite <- nlctx_stack_context. rewrite <- nlctx_app_context.
     change (tConst c' u) with (nl (tConst c' u)).
-    eapply cored_nl.
+    eapply cored_nl ; auto.
     eapply cored_const. eassumption.
   Qed.
   Next Obligation.
@@ -2700,14 +1122,14 @@ Section Conversion.
     eapply red_zippx. eapply red_const. eassumption.
   Qed.
   Next Obligation.
-    eapply red_welltyped ; [ exact h1 | ].
+    eapply red_welltyped ; auto ; [ exact h1 | ].
     constructor. eapply red_zipx. eapply red_const. eassumption.
   Qed.
   Next Obligation.
     left. simpl. eapply cored_zipx.
     rewrite <- nlctx_stack_context. rewrite <- nlctx_app_context.
     change (tConst c' u) with (nl (tConst c' u)).
-    eapply cored_nl.
+    eapply cored_nl ; auto.
     eapply cored_const. eassumption.
   Qed.
   Next Obligation.
@@ -2724,7 +1146,7 @@ Section Conversion.
     (* apply andP in eq1 as [eq1 ec]. *)
     (* apply andP in eq1 as [eq1 ep]. *)
     (* apply andP in eq1 as [eind epar]. *)
-    eapply welltyped_rename ; [ exact h2 |].
+    eapply welltyped_rename ; auto ; [ exact h2 |].
     eapply eq_term_sym.
     eapply eq_term_zipx.
     (* rewrite eq1. reflexivity. *)
@@ -2757,7 +1179,7 @@ Section Conversion.
     eapply conv_conv.
     destruct h. constructor.
     eapply conv_trans ; try eassumption.
-    eapply conv_zippx.
+    eapply conv_zippx ; auto.
     eapply eq_term_conv.
     symmetry in eq1. (* simpl. rewrite eq1. reflexivity. *)
   (* Qed. *)
@@ -2778,7 +1200,7 @@ Section Conversion.
     eexists. eassumption.
   Qed.
   Next Obligation.
-    eapply red_welltyped.
+    eapply red_welltyped ; auto.
     - exact h1.
     - match goal with
       | |- context [ reduce_term ?f ?Σ ?Γ ?t ?h ] =>
@@ -2796,7 +1218,7 @@ Section Conversion.
         * eapply IHbrs.
   Qed.
   Next Obligation.
-    eapply red_welltyped.
+    eapply red_welltyped ; auto.
     - exact h2.
     - match goal with
       | |- context [ reduce_term ?f ?Σ ?Γ ?t ?h ] =>
@@ -2835,8 +1257,7 @@ Section Conversion.
           -- simpl. unfold reduce_term. rewrite e. reflexivity.
           -- simpl. eapply cored_zipx. eapply cored_case.
              rewrite <- nlctx_stack_context. rewrite <- nlctx_app_context.
-             eapply cored_nl.
-             assumption.
+             eapply cored_nl ; auto.
         * exfalso.
           destruct y'. simpl in H0. inversion H0. subst.
           unfold reduce_term in eq3.
@@ -2849,8 +1270,7 @@ Section Conversion.
       + left. simpl.
         eapply cored_zipx. eapply cored_case.
         rewrite <- nlctx_stack_context. rewrite <- nlctx_app_context.
-        eapply cored_nl.
-        assumption.
+        eapply cored_nl ; auto.
       + match goal with
         | |- context [ reduce_term ?f ?Σ ?Γ c' ?h ] =>
           destruct (reduce_stack_Req f Σ Γ c' ε h) as [e' | hr]
@@ -2871,8 +1291,7 @@ Section Conversion.
                 rewrite <- H3. reflexivity.
              ++ simpl. eapply cored_zipx. eapply cored_case.
                 rewrite <- nlctx_stack_context. rewrite <- nlctx_app_context.
-                eapply cored_nl.
-                assumption.
+                eapply cored_nl ; auto.
           -- exfalso.
              destruct y'. simpl in H0. inversion H0. subst.
              destruct y'0. simpl in H2. inversion H2. subst.
@@ -2922,7 +1341,7 @@ Section Conversion.
 
   (* tProj *)
   Next Obligation.
-    eapply welltyped_rename.
+    eapply welltyped_rename ; auto.
     - exact h2.
     - apply eq_term_sym.
       cbn. (* rewrite eq_term_zipx. cbn. *)
@@ -2946,7 +1365,7 @@ Section Conversion.
     eapply conv_conv.
     destruct h. constructor.
     eapply conv_trans ; try eassumption.
-    eapply conv_zippx.
+    eapply conv_zippx ; auto.
     eapply eq_term_conv.
     (* symmetry. assumption. *)
     admit.
@@ -2955,7 +1374,7 @@ Section Conversion.
 
   (* tFix *)
   Next Obligation.
-    eapply welltyped_rename.
+    eapply welltyped_rename ; auto.
     - exact h2.
     - apply eq_term_sym. (* rewrite eq_term_zipx. cbn. rewrite <- eq1. reflexivity. *)
   (* Qed. *)
@@ -2977,7 +1396,7 @@ Section Conversion.
     eapply conv_conv.
     constructor.
     eapply conv_trans ; try eassumption.
-    eapply conv_zippx.
+    eapply conv_zippx ; auto.
     eapply eq_term_conv.
     (* symmetry. assumption. *)
   (* Qed. *)
@@ -2989,11 +1408,11 @@ Section Conversion.
     rewrite <- eq2 in r.
     case_eq (decompose_stack π1). intros l1 ρ1 e1.
     rewrite e1 in r.
-    apply welltyped_zipx in h1 as hh1.
-    apply welltyped_zipc_zippx in hh1.
+    apply welltyped_zipx in h1 as hh1 ; auto.
+    apply welltyped_zipc_zippx in hh1 ; auto.
     pose proof (decompose_stack_eq _ _ _ e1). subst.
     unfold zippx in hh1. rewrite e1 in hh1.
-    pose proof (red_welltyped hh1 r) as hh.
+    pose proof (red_welltyped flags _ hh1 r) as hh.
     apply welltyped_it_mkLambda_or_LetIn in hh.
     assumption.
   Qed.
@@ -3014,12 +1433,12 @@ Section Conversion.
     case_eq (decompose_stack ρ). intros l ξ e.
     rewrite e in d2. cbn in d2. subst.
     apply welltyped_zipx in h1 as hh1.
-    pose proof (red_welltyped hh1 r1) as hh.
+    pose proof (red_welltyped flags _ hh1 r1) as hh.
     apply red_context in r2.
     pose proof (decompose_stack_eq _ _ _ (eq_sym eq2)). subst.
     rewrite zipc_appstack in hh. cbn in r2.
-    pose proof (red_welltyped hh (sq _ r2)) as hh2.
-    eapply zipx_welltyped.
+    pose proof (red_welltyped flags _ hh (sq _ r2)) as hh2.
+    eapply zipx_welltyped ; auto.
     rewrite zipc_stack_cat.
     assumption.
   Qed.
@@ -3033,11 +1452,11 @@ Section Conversion.
     rewrite <- eq3 in r2.
     left. simpl. eapply cored_it_mkLambda_or_LetIn.
     rewrite app_context_nil_l.
-    apply cored_nl in r1.
+    apply cored_nl in r1 ; auto.
     rewrite 2!nl_zipc in r1. cbn in r1.
     eapply red_cored_cored ; try eassumption.
     apply red_context in r2. cbn in r2.
-    apply red_nl in r2.
+    apply red_nl in r2 ; auto.
     rewrite 4!nl_zipc in r2. rewrite nlstack_appstack in r2.
     cbn in r2.
     rewrite nlstack_cat.
@@ -3098,7 +1517,7 @@ Section Conversion.
       rewrite app_nil_r.
       assumption.
     }
-    pose proof (red_trans _ _ _ _ r1 r2') as r.
+    pose proof (red_trans _ _ _ _ _ r1 r2') as r.
     eapply conv_trans'.
     - eapply red_conv_l. eassumption.
     - assumption.
@@ -3111,10 +1530,10 @@ Section Conversion.
     case_eq (decompose_stack π2). intros l2 ρ2 e2.
     rewrite e2 in r.
     apply welltyped_zipx in h2 as hh2.
-    apply welltyped_zipc_zippx in hh2.
+    apply welltyped_zipc_zippx in hh2 ; auto.
     pose proof (decompose_stack_eq _ _ _ e2). subst.
     unfold zippx in hh2. rewrite e2 in hh2.
-    pose proof (red_welltyped hh2 r) as hh.
+    pose proof (red_welltyped flags _ hh2 r) as hh.
     apply welltyped_it_mkLambda_or_LetIn in hh.
     assumption.
   Qed.
@@ -3135,12 +1554,12 @@ Section Conversion.
     case_eq (decompose_stack ρ). intros l ξ e.
     rewrite e in d2. cbn in d2. subst.
     apply welltyped_zipx in h2 as hh2.
-    pose proof (red_welltyped hh2 r1) as hh.
+    pose proof (red_welltyped flags _ hh2 r1) as hh.
     apply red_context in r2.
     pose proof (decompose_stack_eq _ _ _ (eq_sym eq2)). subst.
     rewrite zipc_appstack in hh. cbn in r2.
-    pose proof (red_welltyped hh (sq _ r2)) as hh'.
-    eapply zipx_welltyped.
+    pose proof (red_welltyped flags _ hh (sq _ r2)) as hh'.
+    eapply zipx_welltyped ; auto.
     rewrite zipc_stack_cat.
     assumption.
   Qed.
@@ -3155,11 +1574,11 @@ Section Conversion.
     eapply R_cored2. all: try reflexivity. simpl.
     eapply cored_it_mkLambda_or_LetIn.
     rewrite app_context_nil_l.
-    apply cored_nl in r1.
+    apply cored_nl in r1 ; auto.
     rewrite 2!nl_zipc in r1. cbn in r1.
     eapply red_cored_cored ; try eassumption.
     apply red_context in r2. cbn in r2.
-    apply red_nl in r2.
+    apply red_nl in r2 ; auto.
     rewrite 4!nl_zipc in r2. rewrite nlstack_appstack in r2.
     cbn in r2.
     rewrite nlstack_cat.
@@ -3219,7 +1638,7 @@ Section Conversion.
       rewrite app_nil_r.
       assumption.
     }
-    pose proof (red_trans _ _ _ _ r1 r2') as r.
+    pose proof (red_trans _ _ _ _ _ r1 r2') as r.
     eapply conv_trans' ; revgoals.
     - eapply red_conv_r. eassumption.
     - assumption.
@@ -3227,7 +1646,7 @@ Section Conversion.
 
   (* tCoFix *)
   Next Obligation.
-    eapply welltyped_rename.
+    eapply welltyped_rename ; auto.
     - exact h2.
     - apply eq_term_sym. (* rewrite eq_term_zipx. cbn. rewrite <- eq1. reflexivity. *)
       admit.
@@ -3246,56 +1665,11 @@ Section Conversion.
     eapply conv_conv.
     destruct h. constructor.
     eapply conv_trans ; try eassumption.
-    eapply conv_zippx.
+    eapply conv_zippx ; auto.
     eapply eq_term_conv.
     (* symmetry. assumption. *)
   (* Qed. *)
   Admitted.
-
-  Lemma positionR_context_position_inv :
-    forall Γ p q,
-      positionR (context_position Γ ++ p) (context_position Γ ++ q) ->
-      positionR p q.
-  Proof.
-    intros Γ p q h.
-    revert p q h.
-    induction Γ as [| [na [b|] A] Γ ih ] ; intros p q h.
-    - assumption.
-    - cbn in h. rewrite <- 2!app_assoc in h. apply ih in h.
-      cbn in h. dependent destruction h.
-      assumption.
-    - cbn in h. rewrite <- 2!app_assoc in h. apply ih in h.
-      cbn in h. dependent destruction h.
-      assumption.
-  Qed.
-
-  Lemma positionR_xposition_inv :
-    forall Γ ρ1 ρ2,
-      positionR (xposition Γ ρ1) (xposition Γ ρ2) ->
-      positionR (stack_position ρ1) (stack_position ρ2).
-  Proof.
-    intros Γ ρ1 ρ2 h.
-    eapply positionR_context_position_inv.
-    eassumption.
-  Qed.
-
-  Lemma it_mkLambda_or_LetIn_inj :
-    forall Γ u v,
-      it_mkLambda_or_LetIn Γ u =
-      it_mkLambda_or_LetIn Γ v ->
-      u = v.
-  Proof.
-    intros Γ u v e.
-    revert u v e.
-    induction Γ as [| [na [b|] A] Γ ih ] ; intros u v e.
-    - assumption.
-    - simpl in e. cbn in e.
-      apply ih in e.
-      inversion e. reflexivity.
-    - simpl in e. cbn in e.
-      apply ih in e.
-      inversion e. reflexivity.
-  Qed.
 
   Definition Aux' Γ t args l1 π1 π2 h2 :=
      forall u1 u2 ca1 a1 ρ2
@@ -3311,7 +1685,7 @@ Section Conversion.
   Axiom cheat : forall {A}, A.
   Tactic Notation "cheat" := exact cheat.
 
-  (* TODO *)
+  (* TODO Subgoal *)
   Lemma conv_ax :
     forall {Γ t args ρ1 args1 u1 l1 ρ2 args2 u2 l2},
       Σ;;; Γ |- it_mkLambda_or_LetIn (stack_context ρ1) u1 =
@@ -3360,7 +1734,7 @@ Section Conversion.
     rewrite <- mkApps_nested.
     destruct H1 as [H1]. unfold zippx in H1.
     simpl in H1. rewrite 2!stack_context_appstack in H1.
-    apply zipx_welltyped.
+    apply zipx_welltyped ; auto.
     clear aux.
     apply welltyped_zipx in h2. cbn in h2. cbn.
     (* We get that u2 is well-typed *)
@@ -3532,7 +1906,7 @@ Section Conversion.
   Qed.
 
   Definition isconv_term Γ leq t1 (h1 : welltyped Σ Γ t1) t2 (h2 : welltyped Σ Γ t2) :=
-    isconv Γ leq t1 ε (zipx_welltyped (π := ε) h1) t2 ε (zipx_welltyped (π := ε) h2).
+    isconv Γ leq t1 ε (zipx_welltyped flags _ hΣ (π := ε) h1) t2 ε (zipx_welltyped flags _ hΣ (π := ε) h2).
 
   Theorem isconv_term_sound :
     forall Γ leq t1 h1 t2 h2,
