pcuic/theories/PCUICSafeLemmata.v
@@ -1,0 +1,1651 @@
+(* Distributed under the terms of the MIT license.   *)
+
+From Coq Require Import Bool String List Program BinPos Compare_dec Arith Lia
+     Classes.RelationClasses Omega.
+From Template Require Import config Universes monad_utils utils BasicAst
+     AstUtils UnivSubst.
+From PCUIC Require Import PCUICAst PCUICAstUtils PCUICInduction PCUICReflect
+     PCUICLiftSubst PCUICUnivSubst PCUICTyping PCUICSafeReduce PCUICCumulativity
+     PCUICSR PCUICPosition PCUICEquality PCUICNameless.
+From Equations Require Import Equations.
+
+Require Import Equations.Prop.DepElim.
+
+Import MonadNotation.
+
+Module PSR := PCUICSafeReduce.
+
+Tactic Notation "zip" "fold" "in" hyp(h) :=
+  lazymatch type of h with
+  | context C[ zipc ?t ?π ] =>
+    let C' := context C[ zip (t,π) ] in
+    change C' in h
+  end.
+
+Tactic Notation "zip" "fold" :=
+  lazymatch goal with
+  | |- context C[ zipc ?t ?π ] =>
+    let C' := context C[ zip (t,π) ] in
+    change C'
+  end.
+
+Inductive conv_pb :=
+| Conv
+| Cumul.
+
+Definition conv leq Σ Γ u v :=
+  match leq with
+  | Conv => ∥ Σ ;;; Γ |- u = v ∥
+  | Cumul => ∥ Σ ;;; Γ |- u <= v ∥
+  end.
+
+Definition nodelta_flags := RedFlags.mk true true true false true true.
+
+Section Lemmata.
+
+  Context (flags : RedFlags.t).
+  Context (Σ : global_context).
+  Context (hΣ : wf Σ).
+
+  Lemma welltyped_rename :
+    forall Γ u v,
+      welltyped Σ Γ u ->
+      eq_term (snd Σ) u v ->
+      welltyped Σ Γ v.
+  Admitted.
+
+  Lemma red_welltyped :
+    forall {Γ u v},
+      welltyped Σ Γ u ->
+      ∥ red (fst Σ) Γ u v ∥ ->
+      welltyped Σ Γ v.
+  Proof.
+    intros Γ u v h [r].
+    revert h. induction r ; intros h.
+    - assumption.
+    - specialize IHr with (1 := ltac:(eassumption)).
+      destruct IHr as [A ?]. exists A.
+      eapply PSR.subject_reduction ; eassumption.
+  Qed.
+
+  Lemma red_cored_or_eq :
+    forall Γ u v,
+      red Σ Γ u v ->
+      cored Σ Γ v u \/ u = v.
+  Proof.
+    intros Γ u v h.
+    induction h.
+    - right. reflexivity.
+    - destruct IHh.
+      + left. eapply cored_trans ; eassumption.
+      + subst. left. constructor. assumption.
+  Qed.
+
+  Set Equations With UIP.
+
+  Lemma cored_it_mkLambda_or_LetIn :
+    forall Γ Δ u v,
+      cored Σ (Γ ,,, Δ) u v ->
+      cored Σ Γ (it_mkLambda_or_LetIn Δ u)
+               (it_mkLambda_or_LetIn Δ v).
+  Proof.
+    intros Γ Δ u v h.
+    induction h.
+    - constructor. apply red1_it_mkLambda_or_LetIn. assumption.
+    - eapply cored_trans.
+      + eapply IHh.
+      + apply red1_it_mkLambda_or_LetIn. assumption.
+  Qed.
+
+  Lemma red_it_mkLambda_or_LetIn :
+    forall Γ Δ u v,
+      red Σ (Γ ,,, Δ) u v ->
+      red Σ Γ (it_mkLambda_or_LetIn Δ u)
+              (it_mkLambda_or_LetIn Δ v).
+  Proof.
+    intros Γ Δ u v h.
+    induction h.
+    - constructor.
+    - econstructor.
+      + eassumption.
+      + eapply red1_it_mkLambda_or_LetIn. assumption.
+  Qed.
+
+  Lemma cored_zipx :
+    forall Γ u v π,
+      cored Σ (Γ ,,, stack_context π) u v ->
+      cored Σ [] (zipx Γ u π) (zipx Γ v π).
+  Proof.
+    intros Γ u v π h.
+    eapply cored_it_mkLambda_or_LetIn.
+    eapply cored_context.
+    rewrite app_context_nil_l.
+    assumption.
+  Qed.
+
+  Lemma red_zipx :
+    forall Γ u v π,
+      red Σ (Γ ,,, stack_context π) u v ->
+      red Σ [] (zipx Γ u π) (zipx Γ v π).
+  Proof.
+    intros Γ u v π h.
+    eapply red_it_mkLambda_or_LetIn.
+    eapply red_context.
+    rewrite app_context_nil_l.
+    assumption.
+  Qed.
+
+  Lemma red_trans :
+    forall Γ u v w,
+      red (fst Σ) Γ u v ->
+      red (fst Σ) Γ v w ->
+      red (fst Σ) Γ u w.
+  Proof.
+    intros Γ u v w h1 h2.
+    revert u h1. induction h2 ; intros u h1.
+    - assumption.
+    - specialize IHh2 with (1 := h1).
+      eapply trans_red.
+      + eapply IHh2.
+      + assumption.
+  Qed.
+
+  Lemma conv_refl' :
+    forall leq Γ t,
+      conv leq Σ Γ t t.
+  Proof.
+    intros leq Γ t.
+    destruct leq.
+    - cbn. constructor. apply conv_refl.
+    - cbn. constructor. apply cumul_refl'.
+  Qed.
+
+  Lemma conv_sym :
+    forall Γ u v,
+      Σ ;;; Γ |- u = v ->
+      Σ ;;; Γ |- v = u.
+  Proof.
+    intros Γ u v [h1 h2].
+    econstructor ; assumption.
+  Qed.
+
+  Lemma conv_conv :
+    forall {Γ leq u v},
+      ∥ Σ ;;; Γ |- u = v ∥ ->
+      conv leq Σ Γ u v.
+  Proof.
+    intros Γ leq u v h.
+    destruct leq.
+    - assumption.
+    - destruct h as [[h1 h2]]. cbn.
+      constructor. assumption.
+  Qed.
+
+  Lemma eq_term_conv :
+    forall {Γ u v},
+      eq_term (snd Σ) u v ->
+      Σ ;;; Γ |- u = v.
+  Proof.
+    intros Γ u v e.
+    constructor.
+    - eapply cumul_refl.
+      eapply eq_term_leq_term. assumption.
+    - eapply cumul_refl.
+      eapply eq_term_leq_term.
+      eapply eq_term_sym.
+      assumption.
+  Qed.
+
+  Lemma conv_trans :
+    forall Γ u v w,
+      Σ ;;; Γ |- u = v ->
+      Σ ;;; Γ |- v = w ->
+      Σ ;;; Γ |- u = w.
+  Proof.
+    intros Γ u v w h1 h2.
+    destruct h1, h2. constructor ; eapply cumul_trans ; eassumption.
+  Qed.
+
+  Lemma conv_trans' :
+    forall leq Γ u v w,
+      conv leq Σ Γ u v ->
+      conv leq Σ Γ v w ->
+      conv leq Σ Γ u w.
+  Proof.
+    intros leq Γ u v w h1 h2.
+    destruct leq.
+    - cbn in *. destruct h1, h2. constructor.
+      eapply conv_trans ; eassumption.
+    - cbn in *. destruct h1, h2. constructor. eapply cumul_trans ; eassumption.
+  Qed.
+
+  Lemma red_conv_l :
+    forall leq Γ u v,
+      red (fst Σ) Γ u v ->
+      conv leq Σ Γ u v.
+  Proof.
+    intros leq Γ u v h.
+    induction h.
+    - apply conv_refl'.
+    - eapply conv_trans' ; try eassumption.
+      destruct leq.
+      + simpl. constructor. constructor.
+        * eapply cumul_red_l.
+          -- eassumption.
+          -- eapply cumul_refl'.
+        * eapply cumul_red_r.
+          -- eapply cumul_refl'.
+          -- assumption.
+      + simpl. constructor.
+        eapply cumul_red_l.
+        * eassumption.
+        * eapply cumul_refl'.
+  Qed.
+
+  Lemma red_conv_r :
+    forall leq Γ u v,
+      red (fst Σ) Γ u v ->
+      conv leq Σ Γ v u.
+  Proof.
+    intros leq Γ u v h.
+    induction h.
+    - apply conv_refl'.
+    - eapply conv_trans' ; try eassumption.
+      destruct leq.
+      + simpl. constructor. constructor.
+        * eapply cumul_red_r.
+          -- eapply cumul_refl'.
+          -- assumption.
+        * eapply cumul_red_l.
+          -- eassumption.
+          -- eapply cumul_refl'.
+      + simpl. constructor.
+        eapply cumul_red_r.
+        * eapply cumul_refl'.
+        * assumption.
+  Qed.
+
+  Lemma conv_conv_l :
+    forall leq Γ u v,
+        Σ ;;; Γ |- u = v ->
+        conv leq Σ Γ u v.
+  Proof.
+    intros [] Γ u v [h1 h2].
+    - cbn. constructor. constructor ; assumption.
+    - cbn. constructor. assumption.
+  Qed.
+
+  Lemma conv_conv_r :
+    forall leq Γ u v,
+        Σ ;;; Γ |- u = v ->
+        conv leq Σ Γ v u.
+  Proof.
+    intros [] Γ u v [h1 h2].
+    - cbn. constructor. constructor ; assumption.
+    - cbn. constructor. assumption.
+  Qed.
+
+  Lemma cumul_App_l :
+    forall {Γ f g x},
+      Σ ;;; Γ |- f <= g ->
+      Σ ;;; Γ |- tApp f x <= tApp g x.
+  Proof.
+    intros Γ f g x h.
+    induction h.
+    - eapply cumul_refl. constructor.
+      + assumption.
+      + apply leq_term_refl.
+    - eapply cumul_red_l ; try eassumption.
+      econstructor. assumption.
+    - eapply cumul_red_r ; try eassumption.
+      econstructor. assumption.
+  Qed.
+
+  Lemma conv_App_r :
+    forall {Γ f x y},
+      Σ ;;; Γ |- x = y ->
+      Σ ;;; Γ |- tApp f x = tApp f y.
+  Proof.
+    intros Γ f x y [h1 h2].
+  Admitted.
+
+  Lemma conv_Prod_l :
+    forall {Γ na A1 A2 B},
+      Σ ;;; Γ |- A1 = A2 ->
+      Σ ;;; Γ |- tProd na A1 B = tProd na A2 B.
+  Proof.
+  Admitted.
+
+  Lemma cumul_Prod_r :
+    forall {Γ na A B1 B2},
+      Σ ;;; Γ ,, vass na A |- B1 <= B2 ->
+      Σ ;;; Γ |- tProd na A B1 <= tProd na A B2.
+  Proof.
+    intros Γ na A B1 B2 h.
+    induction h.
+    - eapply cumul_refl. constructor.
+      + apply leq_term_refl.
+      + assumption.
+    - eapply cumul_red_l ; try eassumption.
+      econstructor. assumption.
+    - eapply cumul_red_r ; try eassumption.
+      econstructor. assumption.
+  Qed.
+
+  Lemma conv_Prod :
+    forall leq Γ na na' A1 A2 B1 B2,
+      Σ ;;; Γ |- A1 = A2 ->
+      conv leq Σ (Γ,, vass na A1) B1 B2 ->
+      conv leq Σ Γ (tProd na A1 B1) (tProd na' A2 B2).
+  Admitted.
+
+  Lemma cumul_context :
+    forall Γ u v ρ,
+      Σ ;;; Γ |- u <= v ->
+      Σ ;;; Γ |- zipc u ρ <= zipc v ρ.
+  Proof.
+    intros Γ u v ρ h.
+    revert u v h. induction ρ ; intros u v h.
+    - cbn. assumption.
+    - cbn. apply IHρ.
+      eapply cumul_App_l. assumption.
+    - cbn. eapply IHρ.
+      (* eapply conv_App_r. *)
+      (* Congruence for application on the right *)
+      admit.
+    - cbn.
+      (* Congruence for case *)
+      admit.
+  Admitted.
+
+  Lemma conv_context :
+    forall Γ u v ρ,
+      Σ ;;; Γ |- u = v ->
+      Σ ;;; Γ |- zipc u ρ = zipc v ρ.
+  Proof.
+    intros Γ u v ρ [].
+    constructor ; eapply cumul_context ; assumption.
+  Qed.
+
+  Lemma conv_context' :
+    forall Γ leq u v ρ,
+      conv leq Σ Γ u v ->
+      conv leq Σ Γ (zipc u ρ) (zipc v ρ).
+  Proof.
+    intros Γ leq u v ρ h.
+    destruct leq.
+    - cbn in *. destruct h as [[h1 h2]]. constructor.
+      constructor ; eapply cumul_context ; assumption.
+    - cbn in *. destruct h. constructor.
+      eapply cumul_context. assumption.
+  Qed.
+
+  Lemma cumul_it_mkLambda_or_LetIn :
+    forall Δ Γ u v,
+      Σ ;;; (Δ ,,, Γ) |- u <= v ->
+      Σ ;;; Δ |- it_mkLambda_or_LetIn Γ u <= it_mkLambda_or_LetIn Γ v.
+  Proof.
+    intros Δ Γ u v h. revert Δ u v h.
+    induction Γ as [| [na [b|] A] Γ ih ] ; intros Δ u v h.
+    - assumption.
+    - simpl. cbn. eapply ih.
+      (* Need cumul for LetIn *)
+      admit.
+    - simpl. cbn. eapply ih.
+      (* Need cumul for Lambda *)
+      admit.
+  Admitted.
+
+  Lemma cumul_zippx :
+    forall Γ u v ρ,
+      Σ ;;; (Γ ,,, stack_context ρ) |- u <= v ->
+      Σ ;;; Γ |- zippx u ρ <= zippx v ρ.
+  Proof.
+    intros Γ u v ρ h.
+    revert u v h. induction ρ ; intros u v h.
+    - cbn. assumption.
+    - unfold zippx. simpl.
+      case_eq (decompose_stack ρ). intros l π e.
+      unfold zippx in IHρ. rewrite e in IHρ.
+      apply IHρ.
+      eapply cumul_App_l. assumption.
+    - unfold zippx. simpl.
+      eapply cumul_it_mkLambda_or_LetIn.
+      assumption.
+    - unfold zippx. simpl.
+      eapply cumul_it_mkLambda_or_LetIn.
+      assumption.
+    - unfold zippx. simpl.
+      eapply cumul_it_mkLambda_or_LetIn.
+      assumption.
+    - unfold zippx. simpl.
+      eapply cumul_it_mkLambda_or_LetIn. cbn.
+      (* Need cumul for Lambda again *)
+      admit.
+    - unfold zippx. simpl.
+      eapply cumul_it_mkLambda_or_LetIn.
+      assumption.
+    - unfold zippx. simpl.
+      eapply cumul_it_mkLambda_or_LetIn. cbn.
+      (* cumul lambda *)
+      admit.
+  Admitted.
+
+  Lemma conv_zippx :
+    forall Γ u v ρ,
+      Σ ;;; Γ ,,, stack_context ρ |- u = v ->
+      Σ ;;; Γ |- zippx u ρ = zippx v ρ.
+  Proof.
+    intros Γ u v ρ [].
+    constructor ; eapply cumul_zippx ; assumption.
+  Qed.
+
+  Lemma conv_zippx' :
+    forall Γ leq u v ρ,
+      conv leq Σ (Γ ,,, stack_context ρ) u v ->
+      conv leq Σ Γ (zippx u ρ) (zippx v ρ).
+  Proof.
+    intros Γ leq u v ρ h.
+    destruct leq.
+    - cbn in *. destruct h as [[h1 h2]]. constructor.
+      constructor ; eapply cumul_zippx ; assumption.
+    - cbn in *. destruct h. constructor.
+      eapply cumul_zippx. assumption.
+  Qed.
+
+    (* TODO MOVE *)
+  Local Ltac lih :=
+    lazymatch goal with
+    | ih : forall v n k, eq_term_upto_univ _ ?u _ -> _
+      |- eq_term_upto_univ _ (lift _ _ ?u) _ =>
+      eapply ih
+    end.
+
+  Lemma eq_term_upto_univ_lift :
+    forall R u v n k,
+      eq_term_upto_univ R u v ->
+      eq_term_upto_univ R (lift n k u) (lift n k v).
+  Proof.
+    intros R u v n k e.
+    induction u in v, n, k, e |- * using term_forall_list_ind.
+    all: dependent destruction e.
+    all: try (cbn ; constructor ; try lih ; assumption).
+    - cbn. destruct (Nat.leb_spec0 k n0).
+      + constructor.
+      + constructor.
+    - cbn. constructor.
+      eapply Forall2_map.
+      eapply Forall2_impl'.
+      + eassumption.
+      + eapply All_Forall.
+        eapply All_impl ; [ eassumption |].
+        intros x H1 y H2. cbn in H1.
+        eapply H1. assumption.
+    - cbn. constructor ; try lih ; try assumption.
+      eapply Forall2_map. eapply Forall2_impl' ; [ eassumption |].
+      eapply All_Forall. eapply All_impl ; [ eassumption |].
+      intros x H0 y [? ?]. cbn in H0. repeat split ; auto.
+      eapply H0. assumption.
+    - cbn. constructor.
+      eapply Forall2_map. eapply Forall2_impl' ; [ eassumption |].
+      eapply All_Forall. eapply All_impl ; [ eassumption |].
+      intros x [h1 h2] y [? [? ?]].
+      repeat split ; auto.
+      + eapply h1. assumption.
+      + apply Forall2_length in H. rewrite H.
+        eapply h2. assumption.
+    - cbn. constructor.
+      eapply Forall2_map. eapply Forall2_impl' ; [ eassumption |].
+      eapply All_Forall. eapply All_impl ; [ eassumption |].
+      intros x [h1 h2] y [? [? ?]].
+      repeat split ; auto.
+      + eapply h1. assumption.
+      + apply Forall2_length in H. rewrite H.
+        eapply h2. assumption.
+  Qed.
+
+  (* TODO MOVE *)
+  Local Ltac sih :=
+    lazymatch goal with
+    | ih : forall v n x y, eq_term_upto_univ _ ?u _ -> _ -> _
+      |- eq_term_upto_univ _ (subst _ _ ?u) _ => eapply ih
+    end.
+
+  (* TODO MOVE *)
+  Lemma eq_term_upto_univ_subst :
+    forall R u v n x y,
+      eq_term_upto_univ R u v ->
+      eq_term_upto_univ R x y ->
+      eq_term_upto_univ R (u{n := x}) (v{n := y}).
+  Proof.
+    intros R u v n x y e1 e2.
+    induction u in v, n, x, y, e1, e2 |- * using term_forall_list_ind.
+    all: dependent destruction e1.
+    all: try (cbn ; constructor ; try sih ; assumption).
+    - cbn. destruct (Nat.leb_spec0 n n0).
+      + destruct (eqb_spec n0 n).
+        * subst. replace (n - n) with 0 by omega. cbn.
+          eapply eq_term_upto_univ_lift. assumption.
+        * replace (n0 - n) with (S (n0 - (S n))) by omega. cbn.
+          rewrite nth_error_nil. constructor.
+      + constructor.
+    - cbn. constructor.
+      eapply Forall2_map. eapply Forall2_impl' ; [ eassumption |].
+      eapply All_Forall.
+      eapply All_impl ; [ eassumption |].
+      intros x0 H1 y0 H2. cbn in H1.
+      eapply H1. all: assumption.
+    - cbn. constructor ; try sih ; try assumption.
+      eapply Forall2_map. eapply Forall2_impl' ; [ eassumption |].
+      eapply All_Forall. eapply All_impl ; [ eassumption |].
+      intros ? H0 ? [? ?]. cbn in H0. repeat split ; auto.
+      eapply H0. all: assumption.
+    - cbn. constructor.
+      eapply Forall2_map. eapply Forall2_impl' ; [ eassumption |].
+      eapply All_Forall. eapply All_impl ; [ eassumption |].
+      intros ? [h1 h2] ? [? [? ?]].
+      repeat split ; auto.
+      + eapply h1. all: assumption.
+      + apply Forall2_length in H. rewrite H.
+        eapply h2. all: assumption.
+    - cbn. constructor.
+      eapply Forall2_map. eapply Forall2_impl' ; [ eassumption |].
+      eapply All_Forall. eapply All_impl ; [ eassumption |].
+      intros ? [h1 h2] ? [? [? ?]].
+      repeat split ; auto.
+      + eapply h1. all: assumption.
+      + apply Forall2_length in H. rewrite H.
+        eapply h2. all: assumption.
+  Qed.
+
+  (* TODO MOVE *)
+  Lemma eq_term_upto_univ_mkApps_l_inv :
+    forall R u l t,
+      eq_term_upto_univ R (mkApps u l) t ->
+      exists u' l',
+        eq_term_upto_univ R u u' /\
+        Forall2 (eq_term_upto_univ R) l l' /\
+        t = mkApps u' l'.
+  Proof.
+    intros R u l t h.
+    induction l in u, t, h |- *.
+    - cbn in h. exists t, []. split ; auto.
+    - cbn in h. apply IHl in h as [u' [l' [h1 [h2 h3]]]].
+      dependent destruction h1. subst.
+      eexists. eexists. split ; [ | split ].
+      + eassumption.
+      + constructor.
+        * eassumption.
+        * eassumption.
+      + cbn. reflexivity.
+  Qed.
+
+  (* TODO MOVE *)
+  Lemma eq_term_upto_univ_mkApps :
+    forall R u1 l1 u2 l2,
+      eq_term_upto_univ R u1 u2 ->
+      Forall2 (eq_term_upto_univ R) l1 l2 ->
+      eq_term_upto_univ R (mkApps u1 l1) (mkApps u2 l2).
+  Proof.
+    intros R u1 l1 u2 l2 hu hl.
+    induction l1 in u1, u2, l2, hu, hl |- *.
+    - inversion hl. subst. assumption.
+    - inversion hl. subst. simpl.
+      eapply IHl1.
+      + constructor. all: assumption.
+      + assumption.
+  Qed.
+
+  (* TODO MOVE *)
+  Lemma Forall2_nth :
+    forall A B P l l' n (d : A) (d' : B),
+      Forall2 P l l' ->
+      P d d' ->
+      P (nth n l d) (nth n l' d').
+  Proof.
+    intros A B P l l' n d d' h hd.
+    induction n in l, l', h |- *.
+    - destruct h.
+      + assumption.
+      + assumption.
+    - destruct h.
+      + assumption.
+      + simpl. apply IHn. assumption.
+  Qed.
+
+  Arguments skipn : simpl nomatch.
+
+  (* TODO MOVE *)
+  Lemma Forall2_skipn :
+    forall A B P l l' n,
+      @Forall2 A B P l l' ->
+      Forall2 P (skipn n l) (skipn n l').
+  Proof.
+    intros A B P l l' n h.
+    induction n in l, l', h |- *.
+    - assumption.
+    - destruct h.
+      + constructor.
+      + simpl. apply IHn. assumption.
+  Qed.
+
+  Lemma Forall2_nth_error_Some_l :
+    forall A B (P : A -> B -> Prop) l l' n t,
+      nth_error l n = Some t ->
+      Forall2 P l l' ->
+      exists t',
+        nth_error l' n = Some t' /\
+        P t t'.
+  Proof.
+    intros A B P l l' n t e h.
+    induction n in l, l', t, e, h |- *.
+    - destruct h.
+      + cbn in e. discriminate.
+      + cbn in e. inversion e. subst.
+        exists y. split ; auto.
+    - destruct h.
+      + cbn in e. discriminate.
+      + cbn in e. apply IHn with (l' := l') in e ; assumption.
+  Qed.
+
+  (* TODO MOVE *)
+  Lemma eq_term_upto_univ_isApp :
+    forall R u v,
+      eq_term_upto_univ R u v ->
+      isApp u = isApp v.
+  Proof.
+    intros R u v h.
+    induction h.
+    all: reflexivity.
+  Qed.
+
+  (* TODO MOVE *)
+  Lemma isApp_mkApps :
+    forall u l,
+      isApp u ->
+      isApp (mkApps u l).
+  Proof.
+    intros u l h.
+    induction l in u, h |- *.
+    - cbn. assumption.
+    - cbn. apply IHl. reflexivity.
+  Qed.
+
+  (* TODO MOVE *)
+  Fixpoint nApp t :=
+    match t with
+    | tApp u _ => S (nApp u)
+    | _ => 0
+    end.
+
+  (* TODO MOVE *)
+  Lemma nApp_mkApps :
+    forall t l,
+      nApp (mkApps t l) = nApp t + #|l|.
+  Proof.
+    intros t l.
+    induction l in t |- *.
+    - simpl. omega.
+    - simpl. rewrite IHl. cbn. omega.
+  Qed.
+
+  (* TODO MOVE *)
+  Lemma mkApps_nApp_inj :
+    forall u u' l l',
+      nApp u = nApp u' ->
+      mkApps u l = mkApps u' l' ->
+      u = u' /\ l = l'.
+  Proof.
+    intros u u' l l' h e.
+    induction l in u, u', l', h, e |- *.
+    - cbn in e. subst.
+      destruct l' ; auto.
+      exfalso.
+      rewrite nApp_mkApps in h. cbn in h. omega.
+    - destruct l'.
+      + cbn in e. subst. exfalso.
+        rewrite nApp_mkApps in h. cbn in h. omega.
+      + cbn in e. apply IHl in e.
+        * destruct e as [e1 e2].
+          inversion e1. subst. auto.
+        * cbn. f_equal. auto.
+  Qed.
+
+  (* TODO MOVE *)
+  Lemma isApp_false_nApp :
+    forall u,
+      isApp u = false ->
+      nApp u = 0.
+  Proof.
+    intros u h.
+    destruct u.
+    all: try reflexivity.
+    discriminate.
+  Qed.
+
+  (* TODO MOVE *)
+  Lemma mkApps_notApp_inj :
+    forall u u' l l',
+      isApp u = false ->
+      isApp u' = false ->
+      mkApps u l = mkApps u' l' ->
+      u = u' /\ l = l'.
+  Proof.
+    intros u u' l l' h h' e.
+    eapply mkApps_nApp_inj.
+    - rewrite 2!isApp_false_nApp by assumption. reflexivity.
+    - assumption.
+  Qed.
+
+  (* TODO MOVE *)
+  Lemma eq_term_upto_univ_mkApps_inv :
+    forall R u l u' l',
+      isApp u = false ->
+      isApp u' = false ->
+      eq_term_upto_univ R (mkApps u l) (mkApps u' l') ->
+      eq_term_upto_univ R u u' /\ Forall2 (eq_term_upto_univ R) l l'.
+  Proof.
+    intros R u l u' l' hu hu' h.
+    apply eq_term_upto_univ_mkApps_l_inv in h as hh.
+    destruct hh as [v [args [h1 [h2 h3]]]].
+    apply eq_term_upto_univ_isApp in h1 as hh1. rewrite hu in hh1.
+    apply mkApps_notApp_inj in h3 ; auto.
+    destruct h3 as [? ?]. subst. split ; auto.
+  Qed.
+
+  (* TODO MOVE *)
+  Lemma decompose_app_rec_notApp :
+    forall t l u l',
+      decompose_app_rec t l = (u, l') ->
+      isApp u = false.
+  Proof.
+    intros t l u l' e.
+    induction t in l, u, l', e |- *.
+    all: try (cbn in e ; inversion e ; reflexivity).
+    cbn in e. eapply IHt1. eassumption.
+  Qed.
+
+  (* TODO MOVE *)
+  Lemma decompose_app_notApp :
+    forall t u l,
+      decompose_app t = (u, l) ->
+      isApp u = false.
+  Proof.
+    intros t u l e.
+    eapply decompose_app_rec_notApp. eassumption.
+  Qed.
+
+  (* TODO MOVE? *)
+  Lemma isConstruct_app_eq_term_l :
+    forall R u v,
+      isConstruct_app u ->
+      eq_term_upto_univ R u v ->
+      isConstruct_app v.
+  Proof.
+    intros R u v h e.
+    case_eq (decompose_app u). intros t1 l1 e1.
+    case_eq (decompose_app v). intros t2 l2 e2.
+    unfold isConstruct_app in *.
+    rewrite e1 in h. cbn in h.
+    rewrite e2. cbn.
+    destruct t1 ; try discriminate.
+    apply PCUICConfluence.decompose_app_inv in e1 as ?. subst.
+    apply PCUICConfluence.decompose_app_inv in e2 as ?. subst.
+    apply eq_term_upto_univ_mkApps_inv in e as hh.
+    - destruct hh as [h1 h2].
+      dependent destruction h1. reflexivity.
+    - reflexivity.
+    - eapply decompose_app_notApp. eassumption.
+  Qed.
+
+  (* TODO MOVE *)
+  (* Subsumes the other lemma? *)
+  Lemma eq_term_upto_univ_substs :
+    forall R u v n l l',
+      eq_term_upto_univ R u v ->
+      Forall2 (eq_term_upto_univ R) l l' ->
+      eq_term_upto_univ R (subst l n u) (subst l' n v).
+  Proof.
+    intros R u v n l l' hu hl.
+    induction u in v, n, l, l', hu, hl |- * using term_forall_list_ind.
+    all: dependent destruction hu.
+    all: try (cbn ; constructor ; try sih ; assumption).
+(*     - cbn. destruct (Nat.leb_spec0 n n0). *)
+(*       + destruct (eqb_spec n0 n). *)
+(*         * subst. replace (n - n) with 0 by omega. *)
+(*           destruct hl. *)
+(*           -- cbn. constructor. *)
+(*           -- cbn. eapply eq_term_upto_univ_lift. assumption. *)
+(*         * replace (n0 - n) with (S (n0 - (S n))) by omega. *)
+(*           destruct hl. *)
+(*           -- cbn. constructor. *)
+(*           -- cbn.  *)
+
+(* induction hl in n |- *. *)
+(*       + rewrite subst_empty. constructor. *)
+(*       + cbn. destruct (Nat.leb_spec0 n n0). *)
+(*         * destruct (eqb_spec n0 n). *)
+(*           -- subst. replace (n - n) with 0 by omega. cbn. *)
+(*              eapply eq_term_upto_univ_lift. assumption. *)
+(*           -- replace (n0 - n) with (S (n0 - (S n))) by omega. cbn. *)
+(*              cbn in IHhl. specialize (IHhl (S n)). *)
+(*              revert IHhl. *)
+(*              destruct (Nat.leb_spec0 (S n) n0) ; try (exfalso ; omega). *)
+(*              case_eq (nth_error l (n0 - S n)). *)
+(*              ++ intros b e. *)
+(*                 case_eq (nth_error l' (n0 - S n)). *)
+(*                 ** intros b' e' ih. *)
+
+
+
+(* cbn. destruct (Nat.leb_spec0 n n0). *)
+(*       + destruct (eqb_spec n0 n). *)
+(*         * subst. replace (n - n) with 0 by omega. *)
+(*           destruct hl. *)
+(*           -- cbn. constructor. *)
+(*           -- cbn. eapply eq_term_upto_univ_lift. assumption. *)
+(*         * replace (n0 - n) with (S (n0 - (S n))) by omega. *)
+(*           destruct hl. *)
+(*           -- cbn. constructor. *)
+(*           -- cbn. *)
+
+(*           eapply eq_term_upto_univ_lift. assumption. *)
+(*         * replace (n0 - n) with (S (n0 - (S n))) by omega. cbn. *)
+(*           rewrite nth_error_nil. constructor. *)
+(*       + constructor. *)
+    - admit.
+    - cbn. constructor.
+      eapply Forall2_map. eapply Forall2_impl' ; [ eassumption |].
+      eapply All_Forall.
+      eapply All_impl ; [ eassumption |].
+      intros x0 H1 y0 H2. cbn in H1.
+      eapply H1. all: assumption.
+    - cbn. constructor ; try sih ; try assumption.
+      eapply Forall2_map. eapply Forall2_impl' ; [ eassumption |].
+      eapply All_Forall. eapply All_impl ; [ eassumption |].
+      intros ? H0 ? [? ?]. cbn in H0. repeat split ; auto.
+      eapply H0. all: assumption.
+    - cbn. constructor.
+      eapply Forall2_map. eapply Forall2_impl' ; [ eassumption |].
+      eapply All_Forall. eapply All_impl ; [ eassumption |].
+      intros ? [h1 h2] ? [? [? ?]].
+      repeat split ; auto.
+      + eapply h1. all: assumption.
+      + apply Forall2_length in H. rewrite H.
+        eapply h2. all: assumption.
+    - cbn. constructor.
+      eapply Forall2_map. eapply Forall2_impl' ; [ eassumption |].
+      eapply All_Forall. eapply All_impl ; [ eassumption |].
+      intros ? [h1 h2] ? [? [? ?]].
+      repeat split ; auto.
+      + eapply h1. all: assumption.
+      + apply Forall2_length in H. rewrite H.
+        eapply h2. all: assumption.
+  Admitted.
+
+  (* TODO MOVE *)
+  Lemma red1_eq_term_upto_univ_l :
+    forall R Γ u v u',
+      Reflexive R ->
+      eq_term_upto_univ R u u' ->
+      red1 Σ Γ u v ->
+      exists v',
+        ∥ red1 Σ Γ u' v' ∥ /\
+        eq_term_upto_univ R v v'.
+  Proof.
+    intros R Γ u v u' hR e h.
+    induction h in u', e |- *.
+    - dependent destruction e. dependent destruction e1.
+      eexists. split.
+      + constructor. constructor.
+      + eapply eq_term_upto_univ_subst ; assumption.
+    - dependent destruction e.
+      eexists. split.
+      + constructor. constructor.
+      + eapply eq_term_upto_univ_subst ; assumption.
+    - dependent destruction e.
+      eexists. split.
+      + constructor. constructor. eassumption.
+      + eapply eq_term_upto_univ_refl. assumption.
+    - dependent destruction e.
+      apply eq_term_upto_univ_mkApps_l_inv in e2 as [? [? [h1 [h2 h3]]]]. subst.
+      dependent destruction h1.
+      eexists. split.
+      + constructor. constructor.
+      + eapply eq_term_upto_univ_mkApps.
+        * eapply Forall2_nth with (P := fun x y => eq_term_upto_univ R (snd x) (snd y)).
+          -- eapply Forall2_impl ; [ eassumption |].
+             intros x y [? ?]. assumption.
+          -- cbn. eapply eq_term_upto_univ_refl. assumption.
+        * eapply Forall2_skipn. assumption.
+    - apply eq_term_upto_univ_mkApps_l_inv in e as [? [? [h1 [h2 h3]]]]. subst.
+      dependent destruction h1.
+      unfold unfold_fix in e0.
+      case_eq (nth_error mfix idx) ;
+        try (intros e ; rewrite e in e0 ; discriminate e0).
+      intros d e. rewrite e in e0. inversion e0. subst. clear e0.
+      eapply Forall2_nth_error_Some_l in H as hh ; try eassumption.
+      destruct hh as [d' [e' [? [? erarg]]]].
+      unfold is_constructor in e1.
+      case_eq (nth_error args (rarg d)) ;
+        try (intros bot ; rewrite bot in e1 ; discriminate e1).
+      intros a ea. rewrite ea in e1.
+      eapply Forall2_nth_error_Some_l in h2 as hh ; try eassumption.
+      destruct hh as [a' [ea' ?]].
+      eexists. split.
+      + constructor. eapply red_fix.
+        * unfold unfold_fix. rewrite e'. reflexivity.
+        * unfold is_constructor. rewrite <- erarg. rewrite ea'.
+          eapply isConstruct_app_eq_term_l ; eassumption.
+      + eapply eq_term_upto_univ_mkApps.
+        * eapply eq_term_upto_univ_substs.
+          -- assumption.
+          --
+  Admitted.
+
+  Lemma cored_eq_term_upto_univ_r :
+    forall R Γ u v u',
+      Reflexive R ->
+      eq_term_upto_univ R u u' ->
+      cored Σ Γ v u ->
+      exists v',
+        cored Σ Γ v' u' /\
+        eq_term_upto_univ R v v'.
+  Proof.
+    intros R Γ u v u' hR e h.
+    induction h.
+    - eapply red1_eq_term_upto_univ_l in X ; try eassumption.
+      destruct X as [v' [[r] e']].
+      exists v'. split ; auto.
+      constructor. assumption.
+    - specialize (IHh e). destruct IHh as [v' [c ev]].
+      eapply red1_eq_term_upto_univ_l in X ; try eassumption.
+      destruct X as [w' [[?] ?]].
+      exists w'. split ; auto.
+      eapply cored_trans ; eauto.
+  Qed.
+
+  Lemma cored_nl :
+    forall Γ u v,
+      cored Σ Γ u v ->
+      cored Σ (nlctx Γ) (nl u) (nl v).
+  Admitted.
+
+  Lemma red_nl :
+    forall Γ u v,
+      red Σ Γ u v ->
+      red Σ (nlctx Γ) (nl u) (nl v).
+  Admitted.
+
+  Fixpoint nlstack (π : stack) : stack :=
+    match π with
+    | ε => ε
+
+    | App u ρ =>
+      App (nl u) (nlstack ρ)
+
+    | Fix f n args ρ =>
+      Fix (map (map_def_anon nl nl) f) n (map nl args) (nlstack ρ)
+
+    | Case indn p brs ρ =>
+      Case indn (nl p) (map (on_snd nl) brs) (nlstack ρ)
+
+    | Prod_l na B ρ =>
+      Prod_l nAnon (nl B) (nlstack ρ)
+
+    | Prod_r na A ρ =>
+      Prod_r nAnon (nl A) (nlstack ρ)
+
+    | Lambda_ty na b ρ =>
+      Lambda_ty nAnon (nl b) (nlstack ρ)
+
+    | Lambda_tm na A ρ =>
+      Lambda_tm nAnon (nl A) (nlstack ρ)
+
+    | coApp t ρ =>
+      coApp (nl t) (nlstack ρ)
+    end.
+
+  Lemma nlstack_appstack :
+    forall args ρ,
+      nlstack (appstack args ρ) = appstack (map nl args) (nlstack ρ).
+  Proof.
+    intros args ρ.
+    induction args in ρ |- *.
+    - reflexivity.
+    - simpl. f_equal. eapply IHargs.
+  Qed.
+
+  Lemma nlstack_cat :
+    forall ρ θ,
+      nlstack (ρ +++ θ) = nlstack ρ +++ nlstack θ.
+  Proof.
+    intros ρ θ.
+    induction ρ in θ |- *.
+    all: solve [ simpl ; rewrite ?IHρ ; reflexivity ].
+  Qed.
+
+  Lemma stack_position_nlstack :
+    forall ρ,
+      stack_position (nlstack ρ) = stack_position ρ.
+  Proof.
+    intros ρ.
+    induction ρ.
+    all: (simpl ; rewrite ?IHρ ; reflexivity).
+  Qed.
+
+  Lemma nl_it_mkLambda_or_LetIn :
+    forall Γ t,
+      nl (it_mkLambda_or_LetIn Γ t) =
+      it_mkLambda_or_LetIn (nlctx Γ) (nl t).
+  Proof.
+    intros Γ t.
+    induction Γ as [| [na [b|] B] Γ ih] in t |- *.
+    - reflexivity.
+    - simpl. cbn. rewrite ih. reflexivity.
+    - simpl. cbn. rewrite ih. reflexivity.
+  Qed.
+
+  Lemma nl_mkApps :
+    forall t l,
+      nl (mkApps t l) = mkApps (nl t) (map nl l).
+  Proof.
+    intros t l.
+    induction l in t |- *.
+    - reflexivity.
+    - simpl. rewrite IHl. reflexivity.
+  Qed.
+
+  Lemma nl_zipc :
+    forall t π,
+      nl (zipc t π) = zipc (nl t) (nlstack π).
+  Proof.
+    intros t π.
+    induction π in t |- *.
+    all: try solve [ simpl ; rewrite ?IHπ ; reflexivity ].
+    simpl. rewrite IHπ. cbn. f_equal.
+    rewrite nl_mkApps. reflexivity.
+  Qed.
+
+  Lemma nl_zipx :
+    forall Γ t π,
+      nl (zipx Γ t π) = zipx (nlctx Γ) (nl t) (nlstack π).
+  Proof.
+    intros Γ t π.
+    unfold zipx. rewrite nl_it_mkLambda_or_LetIn. f_equal.
+    apply nl_zipc.
+  Qed.
+
+  Lemma nlctx_app_context :
+    forall Γ Δ,
+      nlctx (Γ ,,, Δ) = nlctx Γ ,,, nlctx Δ.
+  Proof.
+    intros Γ Δ.
+    induction Δ as [| [na [b|] B] Δ ih] in Γ |- *.
+    - reflexivity.
+    - simpl. f_equal. apply ih.
+    - simpl. f_equal. apply ih.
+  Qed.
+
+  Lemma nlctx_stack_context :
+    forall ρ,
+      nlctx (stack_context ρ) = stack_context (nlstack ρ).
+  Proof.
+    intro ρ. induction ρ.
+    all: (simpl ; rewrite ?IHρ ; reflexivity).
+  Qed.
+
+  Lemma wf_fun :
+    forall A (R : A -> A -> Prop) B (f : B -> A),
+      well_founded R ->
+      well_founded (fun x y => R (f x) (f y)).
+  Proof.
+    intros A R B f h x.
+    specialize (h (f x)).
+    dependent induction h.
+    constructor. intros y h.
+    eapply H0 ; try reflexivity. assumption.
+  Qed.
+
+  Lemma Acc_fun :
+    forall A (R : A -> A -> Prop) B (f : B -> A) x,
+      Acc R (f x) ->
+      Acc (fun x y => R (f x) (f y)) x.
+  Proof.
+    intros A R B f x h.
+    dependent induction h.
+    constructor. intros y h.
+    eapply H0 ; try reflexivity. assumption.
+  Qed.
+
+    Lemma inversion_LetIn :
+    forall {Γ na b B t T},
+      Σ ;;; Γ |- tLetIn na b B t : T ->
+      exists s1 A,
+        ∥ Σ ;;; Γ |- B : tSort s1 ∥ /\
+        ∥ Σ ;;; Γ |- b : B ∥ /\
+        ∥ Σ ;;; Γ ,, vdef na b B |- t : A ∥ /\
+        ∥ Σ ;;; Γ |- tLetIn na b B A <= T ∥.
+  Proof.
+    intros Γ na b B t T h. dependent induction h.
+    - exists s1, b'_ty. split ; [| split ; [| split]].
+      + constructor. assumption.
+      + constructor. assumption.
+      + constructor. assumption.
+      + constructor. apply cumul_refl'.
+    - destruct IHh as [s1 [A' [? [? [? hc]]]]].
+      exists s1, A'. split ; [| split ; [| split]].
+      all: try assumption.
+      destruct hc.
+      constructor. eapply cumul_trans ; eassumption.
+  Qed.
+
+  Lemma welltyped_it_mkLambda_or_LetIn :
+    forall Γ Δ t,
+      welltyped Σ Γ (it_mkLambda_or_LetIn Δ t) ->
+      welltyped Σ (Γ ,,, Δ) t.
+  Proof.
+    intros Γ Δ t h.
+    revert Γ t h.
+    induction Δ as [| [na [b|] A] Δ ih ] ; intros Γ t h.
+    - assumption.
+    - simpl. apply ih in h. cbn in h.
+      destruct h as [T h].
+      pose proof (inversion_LetIn h) as [s1 [A' [[?] [[?] [[?] [?]]]]]].
+      exists A'. assumption.
+    - simpl. apply ih in h. cbn in h.
+      destruct h as [T h].
+      pose proof (inversion_Lambda h) as [s1 [B [[?] [[?] [?]]]]].
+      exists B. assumption.
+  Qed.
+
+  Lemma welltyped_zipp :
+    forall Γ t ρ,
+      welltyped Σ Γ (zipp t ρ) ->
+      welltyped Σ Γ t.
+  Proof.
+    intros Γ t ρ [A h].
+    unfold zipp in h.
+    case_eq (decompose_stack ρ). intros l π e.
+    rewrite e in h. clear - h.
+    revert t A h.
+    induction l ; intros t A h.
+    - eexists. cbn in h. eassumption.
+    - cbn in h. apply IHl in h.
+      destruct h as [T h].
+      destruct (inversion_App h) as [na [A' [B' [[?] [[?] [?]]]]]].
+      eexists. eassumption.
+  Qed.
+
+  Lemma welltyped_zippx :
+    forall Γ t ρ,
+      welltyped Σ Γ (zippx t ρ) ->
+      welltyped Σ (Γ ,,, stack_context ρ) t.
+  Proof.
+    intros Γ t ρ h.
+    unfold zippx in h.
+    case_eq (decompose_stack ρ). intros l π e.
+    rewrite e in h.
+    apply welltyped_it_mkLambda_or_LetIn in h.
+    pose proof (decompose_stack_eq _ _ _ e). subst.
+    rewrite stack_context_appstack.
+    clear - h. destruct h as [A h].
+    revert t A h.
+    induction l ; intros t A h.
+    - eexists. eassumption.
+    - cbn in h. apply IHl in h.
+      destruct h as [B h].
+      destruct (inversion_App h) as [na [A' [B' [[?] [[?] [?]]]]]].
+      eexists. eassumption.
+  Qed.
+
+  Derive NoConfusion NoConfusionHom for list.
+
+  Lemma it_mkLambda_or_LetIn_welltyped :
+    forall Γ Δ t,
+      welltyped Σ (Γ ,,, Δ) t ->
+      welltyped Σ Γ (it_mkLambda_or_LetIn Δ t).
+  Proof.
+    intros Γ Δ t h.
+    revert Γ t h.
+    induction Δ as [| [na [b|] B] Δ ih ] ; intros Γ t h.
+    - assumption.
+    - simpl. eapply ih. cbn.
+      destruct h as [A h].
+      pose proof (typing_wf_local h) as hc.
+      cbn in hc. dependent destruction hc.
+      + cbn in H. inversion H.
+      + cbn in H. symmetry in H. inversion H. subst. clear H.
+        cbn in l.
+        eexists. econstructor ; try eassumption.
+        (* FIXME We need to sort B, but we only know it's a type.
+           It might be a problem with the way context are wellformed.
+           Let typing asks for the type to be sorted so it should
+           also hold in the context.
+           At least they should be synchronised.
+         *)
+        admit.
+    - simpl. eapply ih. cbn.
+      destruct h as [A h].
+      pose proof (typing_wf_local h) as hc.
+      cbn in hc. dependent destruction hc.
+      + cbn in H. symmetry in H. inversion H. subst. clear H.
+        destruct l as [s hs].
+        eexists. econstructor ; eassumption.
+      + cbn in H. inversion H.
+  Admitted.
+
+  Lemma zipx_welltyped :
+    forall {Γ t π},
+      welltyped Σ Γ (zipc t π) ->
+      welltyped Σ [] (zipx Γ t π).
+  Proof.
+    intros Γ t π h.
+    eapply it_mkLambda_or_LetIn_welltyped.
+    rewrite app_context_nil_l.
+    assumption.
+  Qed.
+
+  Lemma welltyped_zipx :
+    forall {Γ t π},
+      welltyped Σ [] (zipx Γ t π) ->
+      welltyped Σ Γ (zipc t π).
+  Proof.
+    intros Γ t π h.
+    apply welltyped_it_mkLambda_or_LetIn in h.
+    rewrite app_context_nil_l in h.
+    assumption.
+  Qed.
+
+  Lemma welltyped_zipc_zippx :
+    forall Γ t π,
+      welltyped Σ Γ (zipc t π) ->
+      welltyped Σ Γ (zippx t π).
+  Proof.
+    intros Γ t π h.
+    unfold zippx.
+    case_eq (decompose_stack π). intros l ρ e.
+    pose proof (decompose_stack_eq _ _ _ e). subst.
+    eapply it_mkLambda_or_LetIn_welltyped.
+    rewrite zipc_appstack in h. zip fold in h.
+    apply welltyped_context in h. assumption.
+  Qed.
+
+  Lemma lookup_env_const_name :
+    forall {c c' d},
+      lookup_env Σ c' = Some (ConstantDecl c d) ->
+      c' = c.
+  Proof.
+    intros c c' d e. clear hΣ.
+    destruct Σ as [Σ' ?]. cbn in e.
+    induction Σ'.
+    - cbn in e. discriminate.
+    - destruct a.
+      + cbn in e. destruct (ident_eq_spec c' k).
+        * subst. inversion e. reflexivity.
+        * apply IHΣ'. assumption.
+      + cbn in e. destruct (ident_eq_spec c' k).
+        * inversion e.
+        * apply IHΣ'. assumption.
+  Qed.
+
+  Lemma red_const :
+    forall {Γ n c u cty cb cu},
+      Some (ConstantDecl n {| cst_type := cty ; cst_body := Some cb ; cst_universes := cu |})
+      = lookup_env Σ c ->
+      red (fst Σ) Γ (tConst c u) (subst_instance_constr u cb).
+  Proof.
+    intros Γ n c u cty cb cu e.
+    symmetry in e.
+    pose proof (lookup_env_const_name e). subst.
+    econstructor.
+    - econstructor.
+    - econstructor.
+      + exact e.
+      + reflexivity.
+  Qed.
+
+  Lemma cored_const :
+    forall {Γ n c u cty cb cu},
+      Some (ConstantDecl n {| cst_type := cty ; cst_body := Some cb ; cst_universes := cu |})
+      = lookup_env Σ c ->
+      cored (fst Σ) Γ (subst_instance_constr u cb) (tConst c u).
+  Proof.
+    intros Γ n c u cty cb cu e.
+    symmetry in e.
+    pose proof (lookup_env_const_name e). subst.
+    econstructor.
+    econstructor.
+    - exact e.
+    - reflexivity.
+  Qed.
+
+  Derive Signature for cumul.
+  Derive Signature for red1.
+
+  Lemma context_conversion :
+    forall {Γ t T Γ'},
+      Σ ;;; Γ |- t : T ->
+      PCUICSR.conv_context Σ Γ Γ' ->
+      Σ ;;; Γ' |- t : T.
+  Admitted.
+
+  Lemma app_reds_r :
+    forall Γ u v1 v2,
+      red Σ Γ v1 v2 ->
+      red Σ Γ (tApp u v1) (tApp u v2).
+  Proof.
+    intros Γ u v1 v2 h.
+    revert u. induction h ; intros u.
+    - constructor.
+    - econstructor.
+      + eapply IHh.
+      + constructor. assumption.
+  Qed.
+
+  Lemma app_cored_r :
+    forall Γ u v1 v2,
+      cored Σ Γ v1 v2 ->
+      cored Σ Γ (tApp u v1) (tApp u v2).
+  Proof.
+    intros Γ u v1 v2 h.
+    induction h.
+    - constructor. constructor. assumption.
+    - eapply cored_trans.
+      + eapply IHh.
+      + constructor. assumption.
+  Qed.
+
+  Lemma cored_red_cored :
+    forall Γ u v w,
+      cored Σ Γ w v ->
+      red Σ Γ u v ->
+      cored Σ Γ w u.
+  Proof.
+    intros Γ u v w h1 h2.
+    revert u h2. induction h1 ; intros t h2.
+    - eapply cored_red_trans ; eassumption.
+    - eapply cored_trans.
+      + eapply IHh1. assumption.
+      + assumption.
+  Qed.
+
+  Lemma red_cored_cored :
+    forall Γ u v w,
+      red Σ Γ v w ->
+      cored Σ Γ v u ->
+      cored Σ Γ w u.
+  Proof.
+    intros Γ u v w h1 h2.
+    revert u h2. induction h1 ; intros t h2.
+    - assumption.
+    - eapply cored_trans.
+      + eapply IHh1. assumption.
+      + assumption.
+  Qed.
+
+  Fixpoint isAppProd (t : term) : bool :=
+    match t with
+    | tApp t l => isAppProd t
+    | tProd na A B => true
+    | _ => false
+    end.
+
+  Fixpoint isProd t :=
+    match t with
+    | tProd na A B => true
+    | _ => false
+    end.
+
+  Lemma isAppProd_isProd :
+    forall Γ t,
+      isAppProd t ->
+      welltyped Σ Γ t ->
+      isProd t.
+  Proof.
+    intros Γ t hp hw.
+    revert Γ hp hw.
+    induction t ; intros Γ hp hw.
+    all: try discriminate hp.
+    - reflexivity.
+    - simpl in hp.
+      specialize IHt1 with (1 := hp).
+      assert (welltyped Σ Γ t1) as h.
+      { destruct hw as [T h].
+        destruct (inversion_App h) as [na [A' [B' [[?] [[?] [?]]]]]].
+        eexists. eassumption.
+      }
+      specialize IHt1 with (1 := h).
+      destruct t1.
+      all: try discriminate IHt1.
+      destruct hw as [T hw'].
+      destruct (inversion_App hw') as [na [A' [B' [[hP] [[?] [?]]]]]].
+      destruct (inversion_Prod hP) as [s1 [s2 [[?] [[?] [bot]]]]].
+      (* dependent destruction bot. *)
+      (* + discriminate e. *)
+      (* + dependent destruction r. *)
+      admit.
+  Admitted.
+
+  Lemma isAppProd_mkApps :
+    forall t l, isAppProd (mkApps t l) = isAppProd t.
+  Proof.
+    intros t l. revert t.
+    induction l ; intros t.
+    - reflexivity.
+    - cbn. rewrite IHl. reflexivity.
+  Qed.
+
+  Lemma isProdmkApps :
+    forall t l,
+      isProd (mkApps t l) ->
+      l = [].
+  Proof.
+    intros t l h.
+    revert t h.
+    induction l ; intros t h.
+    - reflexivity.
+    - cbn in h. specialize IHl with (1 := h). subst.
+      cbn in h. discriminate h.
+  Qed.
+
+  Lemma mkApps_Prod_nil :
+    forall Γ na A B l,
+      welltyped Σ Γ (mkApps (tProd na A B) l) ->
+      l = [].
+  Proof.
+    intros Γ na A B l h.
+    pose proof (isAppProd_isProd) as hh.
+    specialize hh with (2 := h).
+    rewrite isAppProd_mkApps in hh.
+    specialize hh with (1 := eq_refl).
+    apply isProdmkApps in hh. assumption.
+  Qed.
+
+  Lemma eq_term_it_mkLambda_or_LetIn_inv :
+    forall Γ u v,
+      eq_term (snd Σ) (it_mkLambda_or_LetIn Γ u) (it_mkLambda_or_LetIn Γ v) ->
+      eq_term (snd Σ) u v.
+  Proof.
+    intros Γ.
+    induction Γ as [| [na [b|] A] Γ ih ] ; intros u v h.
+    - assumption.
+    - simpl in h. cbn in h. apply ih in h. inversion h. subst.
+      assumption.
+    - simpl in h. cbn in h. apply ih in h. inversion h. subst.
+      assumption.
+  Qed.
+
+  Lemma eq_term_zipc_inv :
+    forall u v π,
+      eq_term (snd Σ) (zipc u π) (zipc v π) ->
+      eq_term (snd Σ) u v.
+  Proof.
+    intros u v π h.
+    revert u v h. induction π ; intros u v h.
+    all: solve [
+      simpl in h ; try apply IHπ in h ;
+      cbn in h ; inversion h ; subst ; assumption
+    ].
+  Qed.
+
+  Lemma eq_term_zipx_inv :
+    forall Γ u v π,
+      eq_term (snd Σ) (zipx Γ u π) (zipx Γ v π) ->
+      eq_term (snd Σ) u v.
+  Proof.
+    intros Γ u v π h.
+    eapply eq_term_zipc_inv.
+    eapply eq_term_it_mkLambda_or_LetIn_inv.
+    eassumption.
+  Qed.
+
+  Lemma eq_term_it_mkLambda_or_LetIn :
+    forall Γ u v,
+      eq_term (snd Σ) u v ->
+      eq_term (snd Σ) (it_mkLambda_or_LetIn Γ u) (it_mkLambda_or_LetIn Γ v).
+  Proof.
+    intros Γ.
+    induction Γ as [| [na [b|] A] Γ ih ] ; intros u v h.
+    - assumption.
+    - simpl. cbn. apply ih. constructor ; try apply eq_term_refl. assumption.
+    - simpl. cbn. apply ih. constructor ; try apply eq_term_refl. assumption.
+  Qed.
+
+  Lemma eq_term_zipc :
+    forall u v π,
+      eq_term (snd Σ) u v ->
+      eq_term (snd Σ) (zipc u π) (zipc v π).
+  Proof.
+    intros u v π h.
+    revert u v h. induction π ; intros u v h.
+    all: try solve [
+      simpl ; try apply IHπ ;
+      cbn ; constructor ; try apply eq_term_refl ; assumption
+    ].
+    - assumption.
+    - simpl. apply IHπ. destruct indn as [i n].
+      constructor.
+      + apply eq_term_refl.
+      + assumption.
+      + eapply Forall_Forall2. eapply Forall_True.
+        intros. split ; auto. apply eq_term_refl.
+  Qed.
+
+  Lemma eq_term_zipx :
+    forall Γ u v π,
+      eq_term (snd Σ) u v ->
+      eq_term (snd Σ) (zipx Γ u π) (zipx Γ v π).
+  Proof.
+    intros Γ u v π h.
+    eapply eq_term_it_mkLambda_or_LetIn.
+    eapply eq_term_zipc.
+    eassumption.
+  Qed.
+
+  (* TODO MOVE or even replace old lemma *)
+  Lemma decompose_stack_noStackApp :
+    forall π l ρ,
+      decompose_stack π = (l,ρ) ->
+      isStackApp ρ = false.
+  Proof.
+    intros π l ρ e.
+    destruct ρ. all: auto.
+    exfalso. eapply decompose_stack_not_app. eassumption.
+  Qed.
+
+  (* TODO MOVE *)
+  Lemma stack_context_decompose :
+    forall π,
+      stack_context (snd (decompose_stack π)) = stack_context π.
+  Proof.
+    intros π.
+    case_eq (decompose_stack π). intros l ρ e.
+    cbn. pose proof (decompose_stack_eq _ _ _ e). subst.
+    rewrite stack_context_appstack. reflexivity.
+  Qed.
+
+  Lemma eq_term_trans :
+    forall G u v w,
+      eq_term G u v ->
+      eq_term G v w ->
+      eq_term G u w.
+  Admitted.
+
+  Lemma nl_subst_instance_constr :
+    forall u b,
+      nl (subst_instance_constr u b) = subst_instance_constr u (nl b).
+  Proof.
+    intros u b.
+    induction b using term_forall_list_ind.
+    all: try (simpl ; rewrite ?IHb, ?IHb1, ?IHb2, ?IHb3 ; reflexivity).
+    - simpl. f_equal. induction H.
+      + reflexivity.
+      + simpl. rewrite p, IHAll. reflexivity.
+    - simpl. rewrite IHb1, IHb2. f_equal.
+      induction X.
+      + reflexivity.
+      + simpl. f_equal.
+        * unfold on_snd. destruct p, x. simpl in *.
+          rewrite p0. reflexivity.
+        * apply IHX.
+    - simpl. f_equal. induction X ; try reflexivity.
+      simpl. rewrite IHX. f_equal.
+      destruct p as [h1 h2].
+      destruct x. simpl in *.
+      unfold map_def, map_def_anon. cbn.
+      rewrite h1, h2. reflexivity.
+    - simpl. f_equal. induction X ; try reflexivity.
+      simpl. rewrite IHX. f_equal.
+      destruct p as [h1 h2].
+      destruct x. simpl in *.
+      unfold map_def, map_def_anon. cbn.
+      rewrite h1, h2. reflexivity.
+  Qed.
+
+  Lemma positionR_context_position_inv :
+    forall Γ p q,
+      positionR (context_position Γ ++ p) (context_position Γ ++ q) ->
+      positionR p q.
+  Proof.
+    intros Γ p q h.
+    revert p q h.
+    induction Γ as [| [na [b|] A] Γ ih ] ; intros p q h.
+    - assumption.
+    - cbn in h. rewrite <- 2!app_assoc in h. apply ih in h.
+      cbn in h. dependent destruction h.
+      assumption.
+    - cbn in h. rewrite <- 2!app_assoc in h. apply ih in h.
+      cbn in h. dependent destruction h.
+      assumption.
+  Qed.
+
+  Lemma positionR_xposition_inv :
+    forall Γ ρ1 ρ2,
+      positionR (xposition Γ ρ1) (xposition Γ ρ2) ->
+      positionR (stack_position ρ1) (stack_position ρ2).
+  Proof.
+    intros Γ ρ1 ρ2 h.
+    eapply positionR_context_position_inv.
+    eassumption.
+  Qed.
+
+  Lemma it_mkLambda_or_LetIn_inj :
+    forall Γ u v,
+      it_mkLambda_or_LetIn Γ u =
+      it_mkLambda_or_LetIn Γ v ->
+      u = v.
+  Proof.
+    intros Γ u v e.
+    revert u v e.
+    induction Γ as [| [na [b|] A] Γ ih ] ; intros u v e.
+    - assumption.
+    - simpl in e. cbn in e.
+      apply ih in e.
+      inversion e. reflexivity.
+    - simpl in e. cbn in e.
+      apply ih in e.
+      inversion e. reflexivity.
+  Qed.
+
+End Lemmata.
